src/FLeXClientFuncsNotations.v
@@ -46,7 +46,7 @@ Import ListNotations.
 
 
 
-Parameter FLeXClient_Ф_constructor : XInteger256 -> TvmCell -> TvmCell -> UExpression PhantomType true . 
+ Parameter FLeXClient_Ф_constructor : XInteger256 -> TvmCell -> TvmCell -> UExpression PhantomType true . 
  Parameter FLeXClient_Ф_setFlexCfg : TonsConfig -> addr_std_compact -> addr_std_compact -> UExpression PhantomType true . 
  Parameter FLeXClient_Ф_setExtWalletCode : TvmCell -> UExpression PhantomType true . 
  Parameter FLeXClient_Ф_setFlexWalletCode : TvmCell -> UExpression PhantomType true . 
@@ -124,130 +124,130 @@ Notation " 'TickTock.tick' " := ( ULState (U:= TickTock ) TickTock_ι_tick ) (in
  Notation " 'TonsConfig.process_queue' " := ( URState (U:= TonsConfig ) TonsConfig_ι_process_queue ) (in custom URValue at level 0) : ursus_scope.
  Notation " 'TonsConfig.send_notify' " := ( ULState (U:= TonsConfig ) TonsConfig_ι_send_notify ) (in custom ULValue at level 0) : ursus_scope.
  Notation " 'TonsConfig.send_notify' " := ( URState (U:= TonsConfig ) TonsConfig_ι_send_notify ) (in custom URValue at level 0) : ursus_scope.
- Notation " 'FLeXClient.owner_' " := ( ULState (U:= FLeXClient ) FLeXClient_ι_owner_ ) (in custom ULValue at level 0) : ursus_scope.
- Notation " 'FLeXClient.owner_' " := ( URState (U:= FLeXClient ) FLeXClient_ι_owner_ ) (in custom URValue at level 0) : ursus_scope.
- Notation " 'FLeXClient.trading_pair_code_' " := ( ULState (U:= FLeXClient ) FLeXClient_ι_trading_pair_code_ ) (in custom ULValue at level 0) : ursus_scope.
- Notation " 'FLeXClient.trading_pair_code_' " := ( URState (U:= FLeXClient ) FLeXClient_ι_trading_pair_code_ ) (in custom URValue at level 0) : ursus_scope.
- Notation " 'FLeXClient.xchg_pair_code_' " := ( ULState (U:= FLeXClient ) FLeXClient_ι_xchg_pair_code_ ) (in custom ULValue at level 0) : ursus_scope.
- Notation " 'FLeXClient.xchg_pair_code_' " := ( URState (U:= FLeXClient ) FLeXClient_ι_xchg_pair_code_ ) (in custom URValue at level 0) : ursus_scope.
- Notation " 'FLeXClient.workchain_id_' " := ( ULState (U:= FLeXClient ) FLeXClient_ι_workchain_id_ ) (in custom ULValue at level 0) : ursus_scope.
- Notation " 'FLeXClient.workchain_id_' " := ( URState (U:= FLeXClient ) FLeXClient_ι_workchain_id_ ) (in custom URValue at level 0) : ursus_scope.
- Notation " 'FLeXClient.tons_cfg_' " := ( ULState (U:= FLeXClient ) FLeXClient_ι_tons_cfg_ ) (in custom ULValue at level 0) : ursus_scope.
- Notation " 'FLeXClient.tons_cfg_' " := ( URState (U:= FLeXClient ) FLeXClient_ι_tons_cfg_ ) (in custom URValue at level 0) : ursus_scope.
- Notation " 'FLeXClient.flex_' " := ( ULState (U:= FLeXClient ) FLeXClient_ι_flex_ ) (in custom ULValue at level 0) : ursus_scope.
- Notation " 'FLeXClient.flex_' " := ( URState (U:= FLeXClient ) FLeXClient_ι_flex_ ) (in custom URValue at level 0) : ursus_scope.
- Notation " 'FLeXClient.notify_addr_' " := ( ULState (U:= FLeXClient ) FLeXClient_ι_notify_addr_ ) (in custom ULValue at level 0) : ursus_scope.
- Notation " 'FLeXClient.notify_addr_' " := ( URState (U:= FLeXClient ) FLeXClient_ι_notify_addr_ ) (in custom URValue at level 0) : ursus_scope.
- Notation " 'FLeXClient.ext_wallet_code_' " := ( ULState (U:= FLeXClient ) FLeXClient_ι_ext_wallet_code_ ) (in custom ULValue at level 0) : ursus_scope.
- Notation " 'FLeXClient.ext_wallet_code_' " := ( URState (U:= FLeXClient ) FLeXClient_ι_ext_wallet_code_ ) (in custom URValue at level 0) : ursus_scope.
- Notation " 'FLeXClient.flex_wallet_code_' " := ( ULState (U:= FLeXClient ) FLeXClient_ι_flex_wallet_code_ ) (in custom ULValue at level 0) : ursus_scope.
- Notation " 'FLeXClient.flex_wallet_code_' " := ( URState (U:= FLeXClient ) FLeXClient_ι_flex_wallet_code_ ) (in custom URValue at level 0) : ursus_scope.
- Notation " 'FLeXClient.flex_wrapper_code_' " := ( ULState (U:= FLeXClient ) FLeXClient_ι_flex_wrapper_code_ ) (in custom ULValue at level 0) : ursus_scope.
- Notation " 'FLeXClient.flex_wrapper_code_' " := ( URState (U:= FLeXClient ) FLeXClient_ι_flex_wrapper_code_ ) (in custom URValue at level 0) : ursus_scope.
- Notation " 'FLeXSellArgsAddrs.my_tip3_addr' " := ( ULState (U:= FLeXSellArgsAddrs ) FLeXSellArgsAddrs_ι_my_tip3_addr ) (in custom ULValue at level 0) : ursus_scope.
- Notation " 'FLeXSellArgsAddrs.my_tip3_addr' " := ( URState (U:= FLeXSellArgsAddrs ) FLeXSellArgsAddrs_ι_my_tip3_addr ) (in custom URValue at level 0) : ursus_scope.
- Notation " 'FLeXSellArgs.price' " := ( ULState (U:= FLeXSellArgs ) FLeXSellArgs_ι_price ) (in custom ULValue at level 0) : ursus_scope.
- Notation " 'FLeXSellArgs.price' " := ( URState (U:= FLeXSellArgs ) FLeXSellArgs_ι_price ) (in custom URValue at level 0) : ursus_scope.
- Notation " 'FLeXSellArgs.amount' " := ( ULState (U:= FLeXSellArgs ) FLeXSellArgs_ι_amount ) (in custom ULValue at level 0) : ursus_scope.
- Notation " 'FLeXSellArgs.amount' " := ( URState (U:= FLeXSellArgs ) FLeXSellArgs_ι_amount ) (in custom URValue at level 0) : ursus_scope.
- Notation " 'FLeXSellArgs.lend_finish_time' " := ( ULState (U:= FLeXSellArgs ) FLeXSellArgs_ι_lend_finish_time ) (in custom ULValue at level 0) : ursus_scope.
- Notation " 'FLeXSellArgs.lend_finish_time' " := ( URState (U:= FLeXSellArgs ) FLeXSellArgs_ι_lend_finish_time ) (in custom URValue at level 0) : ursus_scope.
- Notation " 'FLeXSellArgs.min_amount' " := ( ULState (U:= FLeXSellArgs ) FLeXSellArgs_ι_min_amount ) (in custom ULValue at level 0) : ursus_scope.
- Notation " 'FLeXSellArgs.min_amount' " := ( URState (U:= FLeXSellArgs ) FLeXSellArgs_ι_min_amount ) (in custom URValue at level 0) : ursus_scope.
- Notation " 'FLeXSellArgs.deals_limit' " := ( ULState (U:= FLeXSellArgs ) FLeXSellArgs_ι_deals_limit ) (in custom ULValue at level 0) : ursus_scope.
- Notation " 'FLeXSellArgs.deals_limit' " := ( URState (U:= FLeXSellArgs ) FLeXSellArgs_ι_deals_limit ) (in custom URValue at level 0) : ursus_scope.
- Notation " 'FLeXSellArgs.tons_value' " := ( ULState (U:= FLeXSellArgs ) FLeXSellArgs_ι_tons_value ) (in custom ULValue at level 0) : ursus_scope.
- Notation " 'FLeXSellArgs.tons_value' " := ( URState (U:= FLeXSellArgs ) FLeXSellArgs_ι_tons_value ) (in custom URValue at level 0) : ursus_scope.
- Notation " 'FLeXSellArgs.price_code' " := ( ULState (U:= FLeXSellArgs ) FLeXSellArgs_ι_price_code ) (in custom ULValue at level 0) : ursus_scope.
- Notation " 'FLeXSellArgs.price_code' " := ( URState (U:= FLeXSellArgs ) FLeXSellArgs_ι_price_code ) (in custom URValue at level 0) : ursus_scope.
- Notation " 'FLeXSellArgs.addrs' " := ( ULState (U:= FLeXSellArgs ) FLeXSellArgs_ι_addrs ) (in custom ULValue at level 0) : ursus_scope.
- Notation " 'FLeXSellArgs.addrs' " := ( URState (U:= FLeXSellArgs ) FLeXSellArgs_ι_addrs ) (in custom URValue at level 0) : ursus_scope.
- Notation " 'FLeXSellArgs.tip3_code' " := ( ULState (U:= FLeXSellArgs ) FLeXSellArgs_ι_tip3_code ) (in custom ULValue at level 0) : ursus_scope.
- Notation " 'FLeXSellArgs.tip3_code' " := ( URState (U:= FLeXSellArgs ) FLeXSellArgs_ι_tip3_code ) (in custom URValue at level 0) : ursus_scope.
- Notation " 'FLeXSellArgs.tip3cfg' " := ( ULState (U:= FLeXSellArgs ) FLeXSellArgs_ι_tip3cfg ) (in custom ULValue at level 0) : ursus_scope.
- Notation " 'FLeXSellArgs.tip3cfg' " := ( URState (U:= FLeXSellArgs ) FLeXSellArgs_ι_tip3cfg ) (in custom URValue at level 0) : ursus_scope.
- Notation " 'FLeXBuyArgs.price' " := ( ULState (U:= FLeXBuyArgs ) FLeXBuyArgs_ι_price ) (in custom ULValue at level 0) : ursus_scope.
- Notation " 'FLeXBuyArgs.price' " := ( URState (U:= FLeXBuyArgs ) FLeXBuyArgs_ι_price ) (in custom URValue at level 0) : ursus_scope.
- Notation " 'FLeXBuyArgs.amount' " := ( ULState (U:= FLeXBuyArgs ) FLeXBuyArgs_ι_amount ) (in custom ULValue at level 0) : ursus_scope.
- Notation " 'FLeXBuyArgs.amount' " := ( URState (U:= FLeXBuyArgs ) FLeXBuyArgs_ι_amount ) (in custom URValue at level 0) : ursus_scope.
- Notation " 'FLeXBuyArgs.order_finish_time' " := ( ULState (U:= FLeXBuyArgs ) FLeXBuyArgs_ι_order_finish_time ) (in custom ULValue at level 0) : ursus_scope.
- Notation " 'FLeXBuyArgs.order_finish_time' " := ( URState (U:= FLeXBuyArgs ) FLeXBuyArgs_ι_order_finish_time ) (in custom URValue at level 0) : ursus_scope.
- Notation " 'FLeXBuyArgs.min_amount' " := ( ULState (U:= FLeXBuyArgs ) FLeXBuyArgs_ι_min_amount ) (in custom ULValue at level 0) : ursus_scope.
- Notation " 'FLeXBuyArgs.min_amount' " := ( URState (U:= FLeXBuyArgs ) FLeXBuyArgs_ι_min_amount ) (in custom URValue at level 0) : ursus_scope.
- Notation " 'FLeXBuyArgs.deals_limit' " := ( ULState (U:= FLeXBuyArgs ) FLeXBuyArgs_ι_deals_limit ) (in custom ULValue at level 0) : ursus_scope.
- Notation " 'FLeXBuyArgs.deals_limit' " := ( URState (U:= FLeXBuyArgs ) FLeXBuyArgs_ι_deals_limit ) (in custom URValue at level 0) : ursus_scope.
- Notation " 'FLeXBuyArgs.deploy_value' " := ( ULState (U:= FLeXBuyArgs ) FLeXBuyArgs_ι_deploy_value ) (in custom ULValue at level 0) : ursus_scope.
- Notation " 'FLeXBuyArgs.deploy_value' " := ( URState (U:= FLeXBuyArgs ) FLeXBuyArgs_ι_deploy_value ) (in custom URValue at level 0) : ursus_scope.
- Notation " 'FLeXBuyArgs.price_code' " := ( ULState (U:= FLeXBuyArgs ) FLeXBuyArgs_ι_price_code ) (in custom ULValue at level 0) : ursus_scope.
- Notation " 'FLeXBuyArgs.price_code' " := ( URState (U:= FLeXBuyArgs ) FLeXBuyArgs_ι_price_code ) (in custom URValue at level 0) : ursus_scope.
- Notation " 'FLeXBuyArgs.my_tip3_addr' " := ( ULState (U:= FLeXBuyArgs ) FLeXBuyArgs_ι_my_tip3_addr ) (in custom ULValue at level 0) : ursus_scope.
- Notation " 'FLeXBuyArgs.my_tip3_addr' " := ( URState (U:= FLeXBuyArgs ) FLeXBuyArgs_ι_my_tip3_addr ) (in custom URValue at level 0) : ursus_scope.
- Notation " 'FLeXBuyArgs.tip3_code' " := ( ULState (U:= FLeXBuyArgs ) FLeXBuyArgs_ι_tip3_code ) (in custom ULValue at level 0) : ursus_scope.
- Notation " 'FLeXBuyArgs.tip3_code' " := ( URState (U:= FLeXBuyArgs ) FLeXBuyArgs_ι_tip3_code ) (in custom URValue at level 0) : ursus_scope.
- Notation " 'FLeXBuyArgs.tip3cfg' " := ( ULState (U:= FLeXBuyArgs ) FLeXBuyArgs_ι_tip3cfg ) (in custom ULValue at level 0) : ursus_scope.
- Notation " 'FLeXBuyArgs.tip3cfg' " := ( URState (U:= FLeXBuyArgs ) FLeXBuyArgs_ι_tip3cfg ) (in custom URValue at level 0) : ursus_scope.
- Notation " 'FLeXXchgCfgs.major_tip3cfg' " := ( ULState (U:= FLeXXchgCfgs ) FLeXXchgCfgs_ι_major_tip3cfg ) (in custom ULValue at level 0) : ursus_scope.
- Notation " 'FLeXXchgCfgs.major_tip3cfg' " := ( URState (U:= FLeXXchgCfgs ) FLeXXchgCfgs_ι_major_tip3cfg ) (in custom URValue at level 0) : ursus_scope.
- Notation " 'FLeXXchgCfgs.minor_tip3cfg' " := ( ULState (U:= FLeXXchgCfgs ) FLeXXchgCfgs_ι_minor_tip3cfg ) (in custom ULValue at level 0) : ursus_scope.
- Notation " 'FLeXXchgCfgs.minor_tip3cfg' " := ( URState (U:= FLeXXchgCfgs ) FLeXXchgCfgs_ι_minor_tip3cfg ) (in custom URValue at level 0) : ursus_scope.
- Notation " 'FLeXXchgArgs.sell' " := ( ULState (U:= FLeXXchgArgs ) FLeXXchgArgs_ι_sell ) (in custom ULValue at level 0) : ursus_scope.
- Notation " 'FLeXXchgArgs.sell' " := ( URState (U:= FLeXXchgArgs ) FLeXXchgArgs_ι_sell ) (in custom URValue at level 0) : ursus_scope.
- Notation " 'FLeXXchgArgs.price_num' " := ( ULState (U:= FLeXXchgArgs ) FLeXXchgArgs_ι_price_num ) (in custom ULValue at level 0) : ursus_scope.
- Notation " 'FLeXXchgArgs.price_num' " := ( URState (U:= FLeXXchgArgs ) FLeXXchgArgs_ι_price_num ) (in custom URValue at level 0) : ursus_scope.
- Notation " 'FLeXXchgArgs.price_denum' " := ( ULState (U:= FLeXXchgArgs ) FLeXXchgArgs_ι_price_denum ) (in custom ULValue at level 0) : ursus_scope.
- Notation " 'FLeXXchgArgs.price_denum' " := ( URState (U:= FLeXXchgArgs ) FLeXXchgArgs_ι_price_denum ) (in custom URValue at level 0) : ursus_scope.
- Notation " 'FLeXXchgArgs.amount' " := ( ULState (U:= FLeXXchgArgs ) FLeXXchgArgs_ι_amount ) (in custom ULValue at level 0) : ursus_scope.
- Notation " 'FLeXXchgArgs.amount' " := ( URState (U:= FLeXXchgArgs ) FLeXXchgArgs_ι_amount ) (in custom URValue at level 0) : ursus_scope.
- Notation " 'FLeXXchgArgs.lend_amount' " := ( ULState (U:= FLeXXchgArgs ) FLeXXchgArgs_ι_lend_amount ) (in custom ULValue at level 0) : ursus_scope.
- Notation " 'FLeXXchgArgs.lend_amount' " := ( URState (U:= FLeXXchgArgs ) FLeXXchgArgs_ι_lend_amount ) (in custom URValue at level 0) : ursus_scope.
- Notation " 'FLeXXchgArgs.lend_finish_time' " := ( ULState (U:= FLeXXchgArgs ) FLeXXchgArgs_ι_lend_finish_time ) (in custom ULValue at level 0) : ursus_scope.
- Notation " 'FLeXXchgArgs.lend_finish_time' " := ( URState (U:= FLeXXchgArgs ) FLeXXchgArgs_ι_lend_finish_time ) (in custom URValue at level 0) : ursus_scope.
- Notation " 'FLeXXchgArgs.min_amount' " := ( ULState (U:= FLeXXchgArgs ) FLeXXchgArgs_ι_min_amount ) (in custom ULValue at level 0) : ursus_scope.
- Notation " 'FLeXXchgArgs.min_amount' " := ( URState (U:= FLeXXchgArgs ) FLeXXchgArgs_ι_min_amount ) (in custom URValue at level 0) : ursus_scope.
- Notation " 'FLeXXchgArgs.deals_limit' " := ( ULState (U:= FLeXXchgArgs ) FLeXXchgArgs_ι_deals_limit ) (in custom ULValue at level 0) : ursus_scope.
- Notation " 'FLeXXchgArgs.deals_limit' " := ( URState (U:= FLeXXchgArgs ) FLeXXchgArgs_ι_deals_limit ) (in custom URValue at level 0) : ursus_scope.
- Notation " 'FLeXXchgArgs.tons_value' " := ( ULState (U:= FLeXXchgArgs ) FLeXXchgArgs_ι_tons_value ) (in custom ULValue at level 0) : ursus_scope.
- Notation " 'FLeXXchgArgs.tons_value' " := ( URState (U:= FLeXXchgArgs ) FLeXXchgArgs_ι_tons_value ) (in custom URValue at level 0) : ursus_scope.
- Notation " 'FLeXXchgArgs.xchg_price_code' " := ( ULState (U:= FLeXXchgArgs ) FLeXXchgArgs_ι_xchg_price_code ) (in custom ULValue at level 0) : ursus_scope.
- Notation " 'FLeXXchgArgs.xchg_price_code' " := ( URState (U:= FLeXXchgArgs ) FLeXXchgArgs_ι_xchg_price_code ) (in custom URValue at level 0) : ursus_scope.
- Notation " 'FLeXXchgArgs.addrs' " := ( ULState (U:= FLeXXchgArgs ) FLeXXchgArgs_ι_addrs ) (in custom ULValue at level 0) : ursus_scope.
- Notation " 'FLeXXchgArgs.addrs' " := ( URState (U:= FLeXXchgArgs ) FLeXXchgArgs_ι_addrs ) (in custom URValue at level 0) : ursus_scope.
- Notation " 'FLeXXchgArgs.tip3_code' " := ( ULState (U:= FLeXXchgArgs ) FLeXXchgArgs_ι_tip3_code ) (in custom ULValue at level 0) : ursus_scope.
- Notation " 'FLeXXchgArgs.tip3_code' " := ( URState (U:= FLeXXchgArgs ) FLeXXchgArgs_ι_tip3_code ) (in custom URValue at level 0) : ursus_scope.
- Notation " 'FLeXXchgArgs.tip3cfgs' " := ( ULState (U:= FLeXXchgArgs ) FLeXXchgArgs_ι_tip3cfgs ) (in custom ULValue at level 0) : ursus_scope.
- Notation " 'FLeXXchgArgs.tip3cfgs' " := ( URState (U:= FLeXXchgArgs ) FLeXXchgArgs_ι_tip3cfgs ) (in custom URValue at level 0) : ursus_scope.
- Notation " 'FLeXCancelArgs.price' " := ( ULState (U:= FLeXCancelArgs ) FLeXCancelArgs_ι_price ) (in custom ULValue at level 0) : ursus_scope.
- Notation " 'FLeXCancelArgs.price' " := ( URState (U:= FLeXCancelArgs ) FLeXCancelArgs_ι_price ) (in custom URValue at level 0) : ursus_scope.
- Notation " 'FLeXCancelArgs.min_amount' " := ( ULState (U:= FLeXCancelArgs ) FLeXCancelArgs_ι_min_amount ) (in custom ULValue at level 0) : ursus_scope.
- Notation " 'FLeXCancelArgs.min_amount' " := ( URState (U:= FLeXCancelArgs ) FLeXCancelArgs_ι_min_amount ) (in custom URValue at level 0) : ursus_scope.
- Notation " 'FLeXCancelArgs.deals_limit' " := ( ULState (U:= FLeXCancelArgs ) FLeXCancelArgs_ι_deals_limit ) (in custom ULValue at level 0) : ursus_scope.
- Notation " 'FLeXCancelArgs.deals_limit' " := ( URState (U:= FLeXCancelArgs ) FLeXCancelArgs_ι_deals_limit ) (in custom URValue at level 0) : ursus_scope.
- Notation " 'FLeXCancelArgs.value' " := ( ULState (U:= FLeXCancelArgs ) FLeXCancelArgs_ι_value ) (in custom ULValue at level 0) : ursus_scope.
- Notation " 'FLeXCancelArgs.value' " := ( URState (U:= FLeXCancelArgs ) FLeXCancelArgs_ι_value ) (in custom URValue at level 0) : ursus_scope.
- Notation " 'FLeXCancelArgs.price_code' " := ( ULState (U:= FLeXCancelArgs ) FLeXCancelArgs_ι_price_code ) (in custom ULValue at level 0) : ursus_scope.
- Notation " 'FLeXCancelArgs.price_code' " := ( URState (U:= FLeXCancelArgs ) FLeXCancelArgs_ι_price_code ) (in custom URValue at level 0) : ursus_scope.
- Notation " 'FLeXCancelArgs.tip3_code' " := ( ULState (U:= FLeXCancelArgs ) FLeXCancelArgs_ι_tip3_code ) (in custom ULValue at level 0) : ursus_scope.
- Notation " 'FLeXCancelArgs.tip3_code' " := ( URState (U:= FLeXCancelArgs ) FLeXCancelArgs_ι_tip3_code ) (in custom URValue at level 0) : ursus_scope.
- Notation " 'FLeXCancelArgs.tip3cfg' " := ( ULState (U:= FLeXCancelArgs ) FLeXCancelArgs_ι_tip3cfg ) (in custom ULValue at level 0) : ursus_scope.
- Notation " 'FLeXCancelArgs.tip3cfg' " := ( URState (U:= FLeXCancelArgs ) FLeXCancelArgs_ι_tip3cfg ) (in custom URValue at level 0) : ursus_scope.
- Notation " 'FLeXXchgCancelArgs.sell' " := ( ULState (U:= FLeXXchgCancelArgs ) FLeXXchgCancelArgs_ι_sell ) (in custom ULValue at level 0) : ursus_scope.
- Notation " 'FLeXXchgCancelArgs.sell' " := ( URState (U:= FLeXXchgCancelArgs ) FLeXXchgCancelArgs_ι_sell ) (in custom URValue at level 0) : ursus_scope.
- Notation " 'FLeXXchgCancelArgs.price_num' " := ( ULState (U:= FLeXXchgCancelArgs ) FLeXXchgCancelArgs_ι_price_num ) (in custom ULValue at level 0) : ursus_scope.
- Notation " 'FLeXXchgCancelArgs.price_num' " := ( URState (U:= FLeXXchgCancelArgs ) FLeXXchgCancelArgs_ι_price_num ) (in custom URValue at level 0) : ursus_scope.
- Notation " 'FLeXXchgCancelArgs.price_denum' " := ( ULState (U:= FLeXXchgCancelArgs ) FLeXXchgCancelArgs_ι_price_denum ) (in custom ULValue at level 0) : ursus_scope.
- Notation " 'FLeXXchgCancelArgs.price_denum' " := ( URState (U:= FLeXXchgCancelArgs ) FLeXXchgCancelArgs_ι_price_denum ) (in custom URValue at level 0) : ursus_scope.
- Notation " 'FLeXXchgCancelArgs.min_amount' " := ( ULState (U:= FLeXXchgCancelArgs ) FLeXXchgCancelArgs_ι_min_amount ) (in custom ULValue at level 0) : ursus_scope.
- Notation " 'FLeXXchgCancelArgs.min_amount' " := ( URState (U:= FLeXXchgCancelArgs ) FLeXXchgCancelArgs_ι_min_amount ) (in custom URValue at level 0) : ursus_scope.
- Notation " 'FLeXXchgCancelArgs.deals_limit' " := ( ULState (U:= FLeXXchgCancelArgs ) FLeXXchgCancelArgs_ι_deals_limit ) (in custom ULValue at level 0) : ursus_scope.
- Notation " 'FLeXXchgCancelArgs.deals_limit' " := ( URState (U:= FLeXXchgCancelArgs ) FLeXXchgCancelArgs_ι_deals_limit ) (in custom URValue at level 0) : ursus_scope.
- Notation " 'FLeXXchgCancelArgs.value' " := ( ULState (U:= FLeXXchgCancelArgs ) FLeXXchgCancelArgs_ι_value ) (in custom ULValue at level 0) : ursus_scope.
- Notation " 'FLeXXchgCancelArgs.value' " := ( URState (U:= FLeXXchgCancelArgs ) FLeXXchgCancelArgs_ι_value ) (in custom URValue at level 0) : ursus_scope.
- Notation " 'FLeXXchgCancelArgs.xchg_price_code' " := ( ULState (U:= FLeXXchgCancelArgs ) FLeXXchgCancelArgs_ι_xchg_price_code ) (in custom ULValue at level 0) : ursus_scope.
- Notation " 'FLeXXchgCancelArgs.xchg_price_code' " := ( URState (U:= FLeXXchgCancelArgs ) FLeXXchgCancelArgs_ι_xchg_price_code ) (in custom URValue at level 0) : ursus_scope.
- Notation " 'FLeXXchgCancelArgs.tip3_code' " := ( ULState (U:= FLeXXchgCancelArgs ) FLeXXchgCancelArgs_ι_tip3_code ) (in custom ULValue at level 0) : ursus_scope.
- Notation " 'FLeXXchgCancelArgs.tip3_code' " := ( URState (U:= FLeXXchgCancelArgs ) FLeXXchgCancelArgs_ι_tip3_code ) (in custom URValue at level 0) : ursus_scope.
- Notation " 'FLeXXchgCancelArgs.tip3cfgs' " := ( ULState (U:= FLeXXchgCancelArgs ) FLeXXchgCancelArgs_ι_tip3cfgs ) (in custom ULValue at level 0) : ursus_scope.
- Notation " 'FLeXXchgCancelArgs.tip3cfgs' " := ( URState (U:= FLeXXchgCancelArgs ) FLeXXchgCancelArgs_ι_tip3cfgs ) (in custom URValue at level 0) : ursus_scope.
+ Notation " 'FlexClient.owner_' " := ( ULState (U:= FLeXClient ) FlexClient_ι_owner_ ) (in custom ULValue at level 0) : ursus_scope.
+ Notation " 'FlexClient.owner_' " := ( URState (U:= FLeXClient ) FlexClient_ι_owner_ ) (in custom URValue at level 0) : ursus_scope.
+ Notation " 'FlexClient.trading_pair_code_' " := ( ULState (U:= FLeXClient ) FlexClient_ι_trading_pair_code_ ) (in custom ULValue at level 0) : ursus_scope.
+ Notation " 'FlexClient.trading_pair_code_' " := ( URState (U:= FLeXClient ) FlexClient_ι_trading_pair_code_ ) (in custom URValue at level 0) : ursus_scope.
+ Notation " 'FlexClient.xchg_pair_code_' " := ( ULState (U:= FLeXClient ) FlexClient_ι_xchg_pair_code_ ) (in custom ULValue at level 0) : ursus_scope.
+ Notation " 'FlexClient.xchg_pair_code_' " := ( URState (U:= FLeXClient ) FlexClient_ι_xchg_pair_code_ ) (in custom URValue at level 0) : ursus_scope.
+ Notation " 'FlexClient.workchain_id_' " := ( ULState (U:= FLeXClient ) FlexClient_ι_workchain_id_ ) (in custom ULValue at level 0) : ursus_scope.
+ Notation " 'FlexClient.workchain_id_' " := ( URState (U:= FLeXClient ) FlexClient_ι_workchain_id_ ) (in custom URValue at level 0) : ursus_scope.
+ Notation " 'FlexClient.tons_cfg_' " := ( ULState (U:= FLeXClient ) FlexClient_ι_tons_cfg_ ) (in custom ULValue at level 0) : ursus_scope.
+ Notation " 'FlexClient.tons_cfg_' " := ( URState (U:= FLeXClient ) FlexClient_ι_tons_cfg_ ) (in custom URValue at level 0) : ursus_scope.
+ Notation " 'FlexClient.flex_' " := ( ULState (U:= FLeXClient ) FlexClient_ι_flex_ ) (in custom ULValue at level 0) : ursus_scope.
+ Notation " 'FlexClient.flex_' " := ( URState (U:= FLeXClient ) FlexClient_ι_flex_ ) (in custom URValue at level 0) : ursus_scope.
+ Notation " 'FlexClient.notify_addr_' " := ( ULState (U:= FLeXClient ) FlexClient_ι_notify_addr_ ) (in custom ULValue at level 0) : ursus_scope.
+ Notation " 'FlexClient.notify_addr_' " := ( URState (U:= FLeXClient ) FlexClient_ι_notify_addr_ ) (in custom URValue at level 0) : ursus_scope.
+ Notation " 'FlexClient.ext_wallet_code_' " := ( ULState (U:= FLeXClient ) FlexClient_ι_ext_wallet_code_ ) (in custom ULValue at level 0) : ursus_scope.
+ Notation " 'FlexClient.ext_wallet_code_' " := ( URState (U:= FLeXClient ) FlexClient_ι_ext_wallet_code_ ) (in custom URValue at level 0) : ursus_scope.
+ Notation " 'FlexClient.flex_wallet_code_' " := ( ULState (U:= FLeXClient ) FlexClient_ι_flex_wallet_code_ ) (in custom ULValue at level 0) : ursus_scope.
+ Notation " 'FlexClient.flex_wallet_code_' " := ( URState (U:= FLeXClient ) FlexClient_ι_flex_wallet_code_ ) (in custom URValue at level 0) : ursus_scope.
+ Notation " 'FlexClient.flex_wrapper_code_' " := ( ULState (U:= FLeXClient ) FlexClient_ι_flex_wrapper_code_ ) (in custom ULValue at level 0) : ursus_scope.
+ Notation " 'FlexClient.flex_wrapper_code_' " := ( URState (U:= FLeXClient ) FlexClient_ι_flex_wrapper_code_ ) (in custom URValue at level 0) : ursus_scope.
+ Notation " 'FlexSellArgsAddrs.my_tip3_addr' " := ( ULState (U:= FLeXSellArgsAddrs ) FlexSellArgsAddrs_ι_my_tip3_addr ) (in custom ULValue at level 0) : ursus_scope.
+ Notation " 'FlexSellArgsAddrs.my_tip3_addr' " := ( URState (U:= FLeXSellArgsAddrs ) FlexSellArgsAddrs_ι_my_tip3_addr ) (in custom URValue at level 0) : ursus_scope.
+ Notation " 'FlexSellArgs.price' " := ( ULState (U:= FLeXSellArgs ) FlexSellArgs_ι_price ) (in custom ULValue at level 0) : ursus_scope.
+ Notation " 'FlexSellArgs.price' " := ( URState (U:= FLeXSellArgs ) FlexSellArgs_ι_price ) (in custom URValue at level 0) : ursus_scope.
+ Notation " 'FlexSellArgs.amount' " := ( ULState (U:= FLeXSellArgs ) FlexSellArgs_ι_amount ) (in custom ULValue at level 0) : ursus_scope.
+ Notation " 'FlexSellArgs.amount' " := ( URState (U:= FLeXSellArgs ) FlexSellArgs_ι_amount ) (in custom URValue at level 0) : ursus_scope.
+ Notation " 'FlexSellArgs.lend_finish_time' " := ( ULState (U:= FLeXSellArgs ) FlexSellArgs_ι_lend_finish_time ) (in custom ULValue at level 0) : ursus_scope.
+ Notation " 'FlexSellArgs.lend_finish_time' " := ( URState (U:= FLeXSellArgs ) FlexSellArgs_ι_lend_finish_time ) (in custom URValue at level 0) : ursus_scope.
+ Notation " 'FlexSellArgs.min_amount' " := ( ULState (U:= FLeXSellArgs ) FlexSellArgs_ι_min_amount ) (in custom ULValue at level 0) : ursus_scope.
+ Notation " 'FlexSellArgs.min_amount' " := ( URState (U:= FLeXSellArgs ) FlexSellArgs_ι_min_amount ) (in custom URValue at level 0) : ursus_scope.
+ Notation " 'FlexSellArgs.deals_limit' " := ( ULState (U:= FLeXSellArgs ) FlexSellArgs_ι_deals_limit ) (in custom ULValue at level 0) : ursus_scope.
+ Notation " 'FlexSellArgs.deals_limit' " := ( URState (U:= FLeXSellArgs ) FlexSellArgs_ι_deals_limit ) (in custom URValue at level 0) : ursus_scope.
+ Notation " 'FlexSellArgs.tons_value' " := ( ULState (U:= FLeXSellArgs ) FlexSellArgs_ι_tons_value ) (in custom ULValue at level 0) : ursus_scope.
+ Notation " 'FlexSellArgs.tons_value' " := ( URState (U:= FLeXSellArgs ) FlexSellArgs_ι_tons_value ) (in custom URValue at level 0) : ursus_scope.
+ Notation " 'FlexSellArgs.price_code' " := ( ULState (U:= FLeXSellArgs ) FlexSellArgs_ι_price_code ) (in custom ULValue at level 0) : ursus_scope.
+ Notation " 'FlexSellArgs.price_code' " := ( URState (U:= FLeXSellArgs ) FlexSellArgs_ι_price_code ) (in custom URValue at level 0) : ursus_scope.
+ Notation " 'FlexSellArgs.addrs' " := ( ULState (U:= FLeXSellArgs ) FlexSellArgs_ι_addrs ) (in custom ULValue at level 0) : ursus_scope.
+ Notation " 'FlexSellArgs.addrs' " := ( URState (U:= FLeXSellArgs ) FlexSellArgs_ι_addrs ) (in custom URValue at level 0) : ursus_scope.
+ Notation " 'FlexSellArgs.tip3_code' " := ( ULState (U:= FLeXSellArgs ) FlexSellArgs_ι_tip3_code ) (in custom ULValue at level 0) : ursus_scope.
+ Notation " 'FlexSellArgs.tip3_code' " := ( URState (U:= FLeXSellArgs ) FlexSellArgs_ι_tip3_code ) (in custom URValue at level 0) : ursus_scope.
+ Notation " 'FlexSellArgs.tip3cfg' " := ( ULState (U:= FLeXSellArgs ) FlexSellArgs_ι_tip3cfg ) (in custom ULValue at level 0) : ursus_scope.
+ Notation " 'FlexSellArgs.tip3cfg' " := ( URState (U:= FLeXSellArgs ) FlexSellArgs_ι_tip3cfg ) (in custom URValue at level 0) : ursus_scope.
+ Notation " 'FlexBuyArgs.price' " := ( ULState (U:= FLeXBuyArgs ) FlexBuyArgs_ι_price ) (in custom ULValue at level 0) : ursus_scope.
+ Notation " 'FlexBuyArgs.price' " := ( URState (U:= FLeXBuyArgs ) FlexBuyArgs_ι_price ) (in custom URValue at level 0) : ursus_scope.
+ Notation " 'FlexBuyArgs.amount' " := ( ULState (U:= FLeXBuyArgs ) FlexBuyArgs_ι_amount ) (in custom ULValue at level 0) : ursus_scope.
+ Notation " 'FlexBuyArgs.amount' " := ( URState (U:= FLeXBuyArgs ) FlexBuyArgs_ι_amount ) (in custom URValue at level 0) : ursus_scope.
+ Notation " 'FlexBuyArgs.order_finish_time' " := ( ULState (U:= FLeXBuyArgs ) FlexBuyArgs_ι_order_finish_time ) (in custom ULValue at level 0) : ursus_scope.
+ Notation " 'FlexBuyArgs.order_finish_time' " := ( URState (U:= FLeXBuyArgs ) FlexBuyArgs_ι_order_finish_time ) (in custom URValue at level 0) : ursus_scope.
+ Notation " 'FlexBuyArgs.min_amount' " := ( ULState (U:= FLeXBuyArgs ) FlexBuyArgs_ι_min_amount ) (in custom ULValue at level 0) : ursus_scope.
+ Notation " 'FlexBuyArgs.min_amount' " := ( URState (U:= FLeXBuyArgs ) FlexBuyArgs_ι_min_amount ) (in custom URValue at level 0) : ursus_scope.
+ Notation " 'FlexBuyArgs.deals_limit' " := ( ULState (U:= FLeXBuyArgs ) FlexBuyArgs_ι_deals_limit ) (in custom ULValue at level 0) : ursus_scope.
+ Notation " 'FlexBuyArgs.deals_limit' " := ( URState (U:= FLeXBuyArgs ) FlexBuyArgs_ι_deals_limit ) (in custom URValue at level 0) : ursus_scope.
+ Notation " 'FlexBuyArgs.deploy_value' " := ( ULState (U:= FLeXBuyArgs ) FlexBuyArgs_ι_deploy_value ) (in custom ULValue at level 0) : ursus_scope.
+ Notation " 'FlexBuyArgs.deploy_value' " := ( URState (U:= FLeXBuyArgs ) FlexBuyArgs_ι_deploy_value ) (in custom URValue at level 0) : ursus_scope.
+ Notation " 'FlexBuyArgs.price_code' " := ( ULState (U:= FLeXBuyArgs ) FlexBuyArgs_ι_price_code ) (in custom ULValue at level 0) : ursus_scope.
+ Notation " 'FlexBuyArgs.price_code' " := ( URState (U:= FLeXBuyArgs ) FlexBuyArgs_ι_price_code ) (in custom URValue at level 0) : ursus_scope.
+ Notation " 'FlexBuyArgs.my_tip3_addr' " := ( ULState (U:= FLeXBuyArgs ) FlexBuyArgs_ι_my_tip3_addr ) (in custom ULValue at level 0) : ursus_scope.
+ Notation " 'FlexBuyArgs.my_tip3_addr' " := ( URState (U:= FLeXBuyArgs ) FlexBuyArgs_ι_my_tip3_addr ) (in custom URValue at level 0) : ursus_scope.
+ Notation " 'FlexBuyArgs.tip3_code' " := ( ULState (U:= FLeXBuyArgs ) FlexBuyArgs_ι_tip3_code ) (in custom ULValue at level 0) : ursus_scope.
+ Notation " 'FlexBuyArgs.tip3_code' " := ( URState (U:= FLeXBuyArgs ) FlexBuyArgs_ι_tip3_code ) (in custom URValue at level 0) : ursus_scope.
+ Notation " 'FlexBuyArgs.tip3cfg' " := ( ULState (U:= FLeXBuyArgs ) FlexBuyArgs_ι_tip3cfg ) (in custom ULValue at level 0) : ursus_scope.
+ Notation " 'FlexBuyArgs.tip3cfg' " := ( URState (U:= FLeXBuyArgs ) FlexBuyArgs_ι_tip3cfg ) (in custom URValue at level 0) : ursus_scope.
+ Notation " 'FlexXchgCfgs.major_tip3cfg' " := ( ULState (U:= FLeXXchgCfgs ) FlexXchgCfgs_ι_major_tip3cfg ) (in custom ULValue at level 0) : ursus_scope.
+ Notation " 'FlexXchgCfgs.major_tip3cfg' " := ( URState (U:= FLeXXchgCfgs ) FlexXchgCfgs_ι_major_tip3cfg ) (in custom URValue at level 0) : ursus_scope.
+ Notation " 'FlexXchgCfgs.minor_tip3cfg' " := ( ULState (U:= FLeXXchgCfgs ) FlexXchgCfgs_ι_minor_tip3cfg ) (in custom ULValue at level 0) : ursus_scope.
+ Notation " 'FlexXchgCfgs.minor_tip3cfg' " := ( URState (U:= FLeXXchgCfgs ) FlexXchgCfgs_ι_minor_tip3cfg ) (in custom URValue at level 0) : ursus_scope.
+ Notation " 'FlexXchgArgs.sell' " := ( ULState (U:= FLeXXchgArgs ) FlexXchgArgs_ι_sell ) (in custom ULValue at level 0) : ursus_scope.
+ Notation " 'FlexXchgArgs.sell' " := ( URState (U:= FLeXXchgArgs ) FlexXchgArgs_ι_sell ) (in custom URValue at level 0) : ursus_scope.
+ Notation " 'FlexXchgArgs.price_num' " := ( ULState (U:= FLeXXchgArgs ) FlexXchgArgs_ι_price_num ) (in custom ULValue at level 0) : ursus_scope.
+ Notation " 'FlexXchgArgs.price_num' " := ( URState (U:= FLeXXchgArgs ) FlexXchgArgs_ι_price_num ) (in custom URValue at level 0) : ursus_scope.
+ Notation " 'FlexXchgArgs.price_denum' " := ( ULState (U:= FLeXXchgArgs ) FlexXchgArgs_ι_price_denum ) (in custom ULValue at level 0) : ursus_scope.
+ Notation " 'FlexXchgArgs.price_denum' " := ( URState (U:= FLeXXchgArgs ) FlexXchgArgs_ι_price_denum ) (in custom URValue at level 0) : ursus_scope.
+ Notation " 'FlexXchgArgs.amount' " := ( ULState (U:= FLeXXchgArgs ) FlexXchgArgs_ι_amount ) (in custom ULValue at level 0) : ursus_scope.
+ Notation " 'FlexXchgArgs.amount' " := ( URState (U:= FLeXXchgArgs ) FlexXchgArgs_ι_amount ) (in custom URValue at level 0) : ursus_scope.
+ Notation " 'FlexXchgArgs.lend_amount' " := ( ULState (U:= FLeXXchgArgs ) FlexXchgArgs_ι_lend_amount ) (in custom ULValue at level 0) : ursus_scope.
+ Notation " 'FlexXchgArgs.lend_amount' " := ( URState (U:= FLeXXchgArgs ) FlexXchgArgs_ι_lend_amount ) (in custom URValue at level 0) : ursus_scope.
+ Notation " 'FlexXchgArgs.lend_finish_time' " := ( ULState (U:= FLeXXchgArgs ) FlexXchgArgs_ι_lend_finish_time ) (in custom ULValue at level 0) : ursus_scope.
+ Notation " 'FlexXchgArgs.lend_finish_time' " := ( URState (U:= FLeXXchgArgs ) FlexXchgArgs_ι_lend_finish_time ) (in custom URValue at level 0) : ursus_scope.
+ Notation " 'FlexXchgArgs.min_amount' " := ( ULState (U:= FLeXXchgArgs ) FlexXchgArgs_ι_min_amount ) (in custom ULValue at level 0) : ursus_scope.
+ Notation " 'FlexXchgArgs.min_amount' " := ( URState (U:= FLeXXchgArgs ) FlexXchgArgs_ι_min_amount ) (in custom URValue at level 0) : ursus_scope.
+ Notation " 'FlexXchgArgs.deals_limit' " := ( ULState (U:= FLeXXchgArgs ) FlexXchgArgs_ι_deals_limit ) (in custom ULValue at level 0) : ursus_scope.
+ Notation " 'FlexXchgArgs.deals_limit' " := ( URState (U:= FLeXXchgArgs ) FlexXchgArgs_ι_deals_limit ) (in custom URValue at level 0) : ursus_scope.
+ Notation " 'FlexXchgArgs.tons_value' " := ( ULState (U:= FLeXXchgArgs ) FlexXchgArgs_ι_tons_value ) (in custom ULValue at level 0) : ursus_scope.
+ Notation " 'FlexXchgArgs.tons_value' " := ( URState (U:= FLeXXchgArgs ) FlexXchgArgs_ι_tons_value ) (in custom URValue at level 0) : ursus_scope.
+ Notation " 'FlexXchgArgs.xchg_price_code' " := ( ULState (U:= FLeXXchgArgs ) FlexXchgArgs_ι_xchg_price_code ) (in custom ULValue at level 0) : ursus_scope.
+ Notation " 'FlexXchgArgs.xchg_price_code' " := ( URState (U:= FLeXXchgArgs ) FlexXchgArgs_ι_xchg_price_code ) (in custom URValue at level 0) : ursus_scope.
+ Notation " 'FlexXchgArgs.addrs' " := ( ULState (U:= FLeXXchgArgs ) FlexXchgArgs_ι_addrs ) (in custom ULValue at level 0) : ursus_scope.
+ Notation " 'FlexXchgArgs.addrs' " := ( URState (U:= FLeXXchgArgs ) FlexXchgArgs_ι_addrs ) (in custom URValue at level 0) : ursus_scope.
+ Notation " 'FlexXchgArgs.tip3_code' " := ( ULState (U:= FLeXXchgArgs ) FlexXchgArgs_ι_tip3_code ) (in custom ULValue at level 0) : ursus_scope.
+ Notation " 'FlexXchgArgs.tip3_code' " := ( URState (U:= FLeXXchgArgs ) FlexXchgArgs_ι_tip3_code ) (in custom URValue at level 0) : ursus_scope.
+ Notation " 'FlexXchgArgs.tip3cfgs' " := ( ULState (U:= FLeXXchgArgs ) FlexXchgArgs_ι_tip3cfgs ) (in custom ULValue at level 0) : ursus_scope.
+ Notation " 'FlexXchgArgs.tip3cfgs' " := ( URState (U:= FLeXXchgArgs ) FlexXchgArgs_ι_tip3cfgs ) (in custom URValue at level 0) : ursus_scope.
+ Notation " 'FlexCancelArgs.price' " := ( ULState (U:= FLeXCancelArgs ) FlexCancelArgs_ι_price ) (in custom ULValue at level 0) : ursus_scope.
+ Notation " 'FlexCancelArgs.price' " := ( URState (U:= FLeXCancelArgs ) FlexCancelArgs_ι_price ) (in custom URValue at level 0) : ursus_scope.
+ Notation " 'FlexCancelArgs.min_amount' " := ( ULState (U:= FLeXCancelArgs ) FlexCancelArgs_ι_min_amount ) (in custom ULValue at level 0) : ursus_scope.
+ Notation " 'FlexCancelArgs.min_amount' " := ( URState (U:= FLeXCancelArgs ) FlexCancelArgs_ι_min_amount ) (in custom URValue at level 0) : ursus_scope.
+ Notation " 'FlexCancelArgs.deals_limit' " := ( ULState (U:= FLeXCancelArgs ) FlexCancelArgs_ι_deals_limit ) (in custom ULValue at level 0) : ursus_scope.
+ Notation " 'FlexCancelArgs.deals_limit' " := ( URState (U:= FLeXCancelArgs ) FlexCancelArgs_ι_deals_limit ) (in custom URValue at level 0) : ursus_scope.
+ Notation " 'FlexCancelArgs.value' " := ( ULState (U:= FLeXCancelArgs ) FlexCancelArgs_ι_value ) (in custom ULValue at level 0) : ursus_scope.
+ Notation " 'FlexCancelArgs.value' " := ( URState (U:= FLeXCancelArgs ) FlexCancelArgs_ι_value ) (in custom URValue at level 0) : ursus_scope.
+ Notation " 'FlexCancelArgs.price_code' " := ( ULState (U:= FLeXCancelArgs ) FlexCancelArgs_ι_price_code ) (in custom ULValue at level 0) : ursus_scope.
+ Notation " 'FlexCancelArgs.price_code' " := ( URState (U:= FLeXCancelArgs ) FlexCancelArgs_ι_price_code ) (in custom URValue at level 0) : ursus_scope.
+ Notation " 'FlexCancelArgs.tip3_code' " := ( ULState (U:= FLeXCancelArgs ) FlexCancelArgs_ι_tip3_code ) (in custom ULValue at level 0) : ursus_scope.
+ Notation " 'FlexCancelArgs.tip3_code' " := ( URState (U:= FLeXCancelArgs ) FlexCancelArgs_ι_tip3_code ) (in custom URValue at level 0) : ursus_scope.
+ Notation " 'FlexCancelArgs.tip3cfg' " := ( ULState (U:= FLeXCancelArgs ) FlexCancelArgs_ι_tip3cfg ) (in custom ULValue at level 0) : ursus_scope.
+ Notation " 'FlexCancelArgs.tip3cfg' " := ( URState (U:= FLeXCancelArgs ) FlexCancelArgs_ι_tip3cfg ) (in custom URValue at level 0) : ursus_scope.
+ Notation " 'FlexXchgCancelArgs.sell' " := ( ULState (U:= FLeXXchgCancelArgs ) FlexXchgCancelArgs_ι_sell ) (in custom ULValue at level 0) : ursus_scope.
+ Notation " 'FlexXchgCancelArgs.sell' " := ( URState (U:= FLeXXchgCancelArgs ) FlexXchgCancelArgs_ι_sell ) (in custom URValue at level 0) : ursus_scope.
+ Notation " 'FlexXchgCancelArgs.price_num' " := ( ULState (U:= FLeXXchgCancelArgs ) FlexXchgCancelArgs_ι_price_num ) (in custom ULValue at level 0) : ursus_scope.
+ Notation " 'FlexXchgCancelArgs.price_num' " := ( URState (U:= FLeXXchgCancelArgs ) FlexXchgCancelArgs_ι_price_num ) (in custom URValue at level 0) : ursus_scope.
+ Notation " 'FlexXchgCancelArgs.price_denum' " := ( ULState (U:= FLeXXchgCancelArgs ) FlexXchgCancelArgs_ι_price_denum ) (in custom ULValue at level 0) : ursus_scope.
+ Notation " 'FlexXchgCancelArgs.price_denum' " := ( URState (U:= FLeXXchgCancelArgs ) FlexXchgCancelArgs_ι_price_denum ) (in custom URValue at level 0) : ursus_scope.
+ Notation " 'FlexXchgCancelArgs.min_amount' " := ( ULState (U:= FLeXXchgCancelArgs ) FlexXchgCancelArgs_ι_min_amount ) (in custom ULValue at level 0) : ursus_scope.
+ Notation " 'FlexXchgCancelArgs.min_amount' " := ( URState (U:= FLeXXchgCancelArgs ) FlexXchgCancelArgs_ι_min_amount ) (in custom URValue at level 0) : ursus_scope.
+ Notation " 'FlexXchgCancelArgs.deals_limit' " := ( ULState (U:= FLeXXchgCancelArgs ) FlexXchgCancelArgs_ι_deals_limit ) (in custom ULValue at level 0) : ursus_scope.
+ Notation " 'FlexXchgCancelArgs.deals_limit' " := ( URState (U:= FLeXXchgCancelArgs ) FlexXchgCancelArgs_ι_deals_limit ) (in custom URValue at level 0) : ursus_scope.
+ Notation " 'FlexXchgCancelArgs.value' " := ( ULState (U:= FLeXXchgCancelArgs ) FlexXchgCancelArgs_ι_value ) (in custom ULValue at level 0) : ursus_scope.
+ Notation " 'FlexXchgCancelArgs.value' " := ( URState (U:= FLeXXchgCancelArgs ) FlexXchgCancelArgs_ι_value ) (in custom URValue at level 0) : ursus_scope.
+ Notation " 'FlexXchgCancelArgs.xchg_price_code' " := ( ULState (U:= FLeXXchgCancelArgs ) FlexXchgCancelArgs_ι_xchg_price_code ) (in custom ULValue at level 0) : ursus_scope.
+ Notation " 'FlexXchgCancelArgs.xchg_price_code' " := ( URState (U:= FLeXXchgCancelArgs ) FlexXchgCancelArgs_ι_xchg_price_code ) (in custom URValue at level 0) : ursus_scope.
+ Notation " 'FlexXchgCancelArgs.tip3_code' " := ( ULState (U:= FLeXXchgCancelArgs ) FlexXchgCancelArgs_ι_tip3_code ) (in custom ULValue at level 0) : ursus_scope.
+ Notation " 'FlexXchgCancelArgs.tip3_code' " := ( URState (U:= FLeXXchgCancelArgs ) FlexXchgCancelArgs_ι_tip3_code ) (in custom URValue at level 0) : ursus_scope.
+ Notation " 'FlexXchgCancelArgs.tip3cfgs' " := ( ULState (U:= FLeXXchgCancelArgs ) FlexXchgCancelArgs_ι_tip3cfgs ) (in custom ULValue at level 0) : ursus_scope.
+ Notation " 'FlexXchgCancelArgs.tip3cfgs' " := ( URState (U:= FLeXXchgCancelArgs ) FlexXchgCancelArgs_ι_tip3cfgs ) (in custom URValue at level 0) : ursus_scope.
  Notation " 'XchgPair.flex_addr_' " := ( ULState (U:= XchgPair ) XchgPair_ι_flex_addr_ ) (in custom ULValue at level 0) : ursus_scope.
  Notation " 'XchgPair.flex_addr_' " := ( URState (U:= XchgPair ) XchgPair_ι_flex_addr_ ) (in custom URValue at level 0) : ursus_scope.
  Notation " 'XchgPair.tip3_major_root_' " := ( ULState (U:= XchgPair ) XchgPair_ι_tip3_major_root_ ) (in custom ULValue at level 0) : ursus_scope.
@@ -444,92 +444,92 @@ Notation " 'error_code::message_sender_is_not_my_owner' " := (sInject error_code
 
 
  Definition FLeXClient_Ф_constructor_call { a1 a2 a3 }  ( pubkey : URValue XInteger256 a1 ) ( trading_pair_code : URValue TvmCell a2 ) ( xchg_pair_code : URValue TvmCell a3 ) : LedgerT ( ControlResult PhantomType true ) := 
- 🏓 ursus_call_with_args ( LedgerableWithArgs := λ3 ) FLeXClient_Ф_constructor 
+ 🏓 ursus_call_with_args ( LedgerableWithArgs := λ3 ) FlexClient_Ф_constructor 
  ( SimpleLedgerableArg URValue {{ Λ "pubkey" }} ( pubkey ) ) 
  ( SimpleLedgerableArg URValue {{ Λ "trading_pair_code" }} ( trading_pair_code ) ) 
  ( SimpleLedgerableArg URValue {{ Λ "xchg_pair_code" }} ( xchg_pair_code ) ) 
  . 
- Notation " 'FLeXClient_Ф_constructor_ref_' '(' pubkey trading_pair_code xchg_pair_code ')' " := 
+ Notation " 'FlexClient_Ф_constructor_ref_' '(' pubkey trading_pair_code xchg_pair_code ')' " := 
  ( FuncallExpression ( FLeXClient_Ф_constructor_call 
  pubkey trading_pair_code xchg_pair_code )) 
- (in custom ULValue at level 0 , pubkey custom ULValue at level 0 
- , trading_pair_code custom ULValue at level 0 
- , xchg_pair_code custom ULValue at level 0 ) : ursus_scope . 
+ (in custom URValue at level 0 , pubkey custom URValue at level 0 
+ , trading_pair_code custom URValue at level 0 
+ , xchg_pair_code custom URValue at level 0 ) : ursus_scope . 
  
  Definition FLeXClient_Ф_setFlexCfg_call { a1 a2 a3 }  ( tons_cfg : URValue TonsConfig a1 ) ( flex : URValue addr_std_compact a2 ) ( notify_addr : URValue addr_std_compact a3 ) : LedgerT ( ControlResult PhantomType true ) := 
- 🏓 ursus_call_with_args ( LedgerableWithArgs := λ3 ) FLeXClient_Ф_setFlexCfg 
+ 🏓 ursus_call_with_args ( LedgerableWithArgs := λ3 ) FlexClient_Ф_setFlexCfg 
  ( SimpleLedgerableArg URValue {{ Λ "tons_cfg" }} ( tons_cfg ) ) 
  ( SimpleLedgerableArg URValue {{ Λ "flex" }} ( flex ) ) 
  ( SimpleLedgerableArg URValue {{ Λ "notify_addr" }} ( notify_addr ) ) 
  . 
- Notation " 'FLeXClient_Ф_setFlexCfg_ref_' '(' tons_cfg flex notify_addr ')' " := 
+ Notation " 'FlexClient_Ф_setFlexCfg_ref_' '(' tons_cfg flex notify_addr ')' " := 
  ( FuncallExpression ( FLeXClient_Ф_setFlexCfg_call 
  tons_cfg flex notify_addr )) 
- (in custom ULValue at level 0 , tons_cfg custom ULValue at level 0 
- , flex custom ULValue at level 0 
- , notify_addr custom ULValue at level 0 ) : ursus_scope . 
+ (in custom ULValue at level 0 , tons_cfg custom URValue at level 0 
+ , flex custom URValue at level 0 
+ , notify_addr custom URValue at level 0 ) : ursus_scope . 
  
  Definition FLeXClient_Ф_setExtWalletCode_call { a1 }  ( ext_wallet_code : URValue TvmCell a1 ) : LedgerT ( ControlResult PhantomType true ) := 
- 🏓 ursus_call_with_args ( LedgerableWithArgs := λ1 ) FLeXClient_Ф_setExtWalletCode 
+ 🏓 ursus_call_with_args ( LedgerableWithArgs := λ1 ) FlexClient_Ф_setExtWalletCode 
  ( SimpleLedgerableArg URValue {{ Λ "ext_wallet_code" }} ( ext_wallet_code ) ) 
  . 
- Notation " 'FLeXClient_Ф_setExtWalletCode_ref_' '(' ext_wallet_code ')' " := 
+ Notation " 'FlexClient_Ф_setExtWalletCode_ref_' '(' ext_wallet_code ')' " := 
  ( FuncallExpression ( FLeXClient_Ф_setExtWalletCode_call 
  ext_wallet_code )) 
- (in custom ULValue at level 0 , ext_wallet_code custom ULValue at level 0 ) : ursus_scope . 
+ (in custom ULValue at level 0 , ext_wallet_code custom URValue at level 0 ) : ursus_scope . 
  
  Definition FLeXClient_Ф_setFlexWalletCode_call { a1 }  ( flex_wallet_code : URValue TvmCell a1 ) : LedgerT ( ControlResult PhantomType true ) := 
- 🏓 ursus_call_with_args ( LedgerableWithArgs := λ1 ) FLeXClient_Ф_setFlexWalletCode 
+ 🏓 ursus_call_with_args ( LedgerableWithArgs := λ1 ) FlexClient_Ф_setFlexWalletCode 
  ( SimpleLedgerableArg URValue {{ Λ "flex_wallet_code" }} ( flex_wallet_code ) ) 
  . 
- Notation " 'FLeXClient_Ф_setFlexWalletCode_ref_' '(' flex_wallet_code ')' " := 
+ Notation " 'FlexClient_Ф_setFlexWalletCode_ref_' '(' flex_wallet_code ')' " := 
  ( FuncallExpression ( FLeXClient_Ф_setFlexWalletCode_call 
  flex_wallet_code )) 
- (in custom ULValue at level 0 , flex_wallet_code custom ULValue at level 0 ) : ursus_scope . 
+ (in custom ULValue at level 0 , flex_wallet_code custom URValue at level 0 ) : ursus_scope . 
  
  Definition FLeXClient_Ф_setFlexWrapperCode_call { a1 }  ( flex_wrapper_code : URValue TvmCell a1 ) : LedgerT ( ControlResult PhantomType true ) := 
- 🏓 ursus_call_with_args ( LedgerableWithArgs := λ1 ) FLeXClient_Ф_setFlexWrapperCode 
+ 🏓 ursus_call_with_args ( LedgerableWithArgs := λ1 ) FlexClient_Ф_setFlexWrapperCode 
  ( SimpleLedgerableArg URValue {{ Λ "flex_wrapper_code" }} ( flex_wrapper_code ) ) 
  . 
- Notation " 'FLeXClient_Ф_setFlexWrapperCode_ref_' '(' flex_wrapper_code ')' " := 
+ Notation " 'FlexClient_Ф_setFlexWrapperCode_ref_' '(' flex_wrapper_code ')' " := 
  ( FuncallExpression ( FLeXClient_Ф_setFlexWrapperCode_call 
  flex_wrapper_code )) 
- (in custom ULValue at level 0 , flex_wrapper_code custom ULValue at level 0 ) : ursus_scope . 
+ (in custom ULValue at level 0 , flex_wrapper_code custom URValue at level 0 ) : ursus_scope . 
  
  Definition FLeXClient_Ф_deployTradingPair_call { a1 a2 a3 a4 }  ( tip3_root : URValue addr_std_compact a1 ) ( deploy_min_value : URValue XInteger128 a2 ) ( deploy_value : URValue XInteger128 a3 ) ( min_trade_amount : URValue XInteger128 a4 ) : LedgerT ( ControlResult XAddress true ) := 
- 🏓 ursus_call_with_args ( LedgerableWithArgs := λ4 ) FLeXClient_Ф_deployTradingPair 
+ 🏓 ursus_call_with_args ( LedgerableWithArgs := λ4 ) FlexClient_Ф_deployTradingPair 
  ( SimpleLedgerableArg URValue {{ Λ "tip3_root" }} ( tip3_root ) ) 
  ( SimpleLedgerableArg URValue {{ Λ "deploy_min_value" }} ( deploy_min_value ) ) 
  ( SimpleLedgerableArg URValue {{ Λ "deploy_value" }} ( deploy_value ) ) 
  ( SimpleLedgerableArg URValue {{ Λ "min_trade_amount" }} ( min_trade_amount ) ) 
  . 
- Notation " 'FLeXClient_Ф_deployTradingPair_ref_' '(' tip3_root deploy_min_value deploy_value min_trade_amount ')' " := 
+ Notation " 'FlexClient_Ф_deployTradingPair_ref_' '(' tip3_root deploy_min_value deploy_value min_trade_amount ')' " := 
  ( URResult ( FLeXClient_Ф_deployTradingPair_call 
  tip3_root deploy_min_value deploy_value min_trade_amount )) 
  (in custom URValue at level 0 , tip3_root custom URValue at level 0 
- , deploy_min_value custom ULValue at level 0 
- , deploy_value custom ULValue at level 0 
- , min_trade_amount custom ULValue at level 0 ) : ursus_scope . 
+ , deploy_min_value custom URValue at level 0 
+ , deploy_value custom URValue at level 0 
+ , min_trade_amount custom URValue at level 0 ) : ursus_scope . 
  
  Definition FLeXClient_Ф_deployXchgPair_call { a1 a2 a3 a4 a5 }  ( tip3_major_root : URValue addr_std_compact a1 ) ( tip3_minor_root : URValue addr_std_compact a2 ) ( deploy_min_value : URValue XInteger128 a3 ) ( deploy_value : URValue XInteger128 a4 ) ( min_trade_amount : URValue XInteger128 a5 ) : LedgerT ( ControlResult XAddress true ) := 
- 🏓 ursus_call_with_args ( LedgerableWithArgs := λ5 ) FLeXClient_Ф_deployXchgPair 
+ 🏓 ursus_call_with_args ( LedgerableWithArgs := λ5 ) FlexClient_Ф_deployXchgPair 
  ( SimpleLedgerableArg URValue {{ Λ "tip3_major_root" }} ( tip3_major_root ) ) 
  ( SimpleLedgerableArg URValue {{ Λ "tip3_minor_root" }} ( tip3_minor_root ) ) 
  ( SimpleLedgerableArg URValue {{ Λ "deploy_min_value" }} ( deploy_min_value ) ) 
  ( SimpleLedgerableArg URValue {{ Λ "deploy_value" }} ( deploy_value ) ) 
  ( SimpleLedgerableArg URValue {{ Λ "min_trade_amount" }} ( min_trade_amount ) ) 
  . 
- Notation " 'FLeXClient_Ф_deployXchgPair_ref_' '(' tip3_major_root tip3_minor_root deploy_min_value deploy_value min_trade_amount ')' " := 
+ Notation " 'FlexClient_Ф_deployXchgPair_ref_' '(' tip3_major_root tip3_minor_root deploy_min_value deploy_value min_trade_amount ')' " := 
  ( URResult ( FLeXClient_Ф_deployXchgPair_call 
  tip3_major_root tip3_minor_root deploy_min_value deploy_value min_trade_amount )) 
  (in custom URValue at level 0 , tip3_major_root custom URValue at level 0 
- , tip3_minor_root custom ULValue at level 0 
- , deploy_min_value custom ULValue at level 0 
- , deploy_value custom ULValue at level 0 
- , min_trade_amount custom ULValue at level 0 ) : ursus_scope . 
+ , tip3_minor_root custom URValue at level 0 
+ , deploy_min_value custom URValue at level 0 
+ , deploy_value custom URValue at level 0 
+ , min_trade_amount custom URValue at level 0 ) : ursus_scope . 
  
  Definition FLeXClient_Ф_preparePrice_call { a1 a2 a3 a4 a5 a6 }  ( price : URValue XInteger128 a1 ) ( min_amount : URValue XInteger128 a2 ) ( deals_limit : URValue XInteger8 a3 ) ( tip3_code : URValue TvmCell a4 ) ( tip3cfg : URValue Tip3Config a5 ) ( price_code : URValue TvmCell a6 ) : LedgerT ( ControlResult ( StateInit # XAddress # XInteger256 ) (orb (orb (orb (orb (orb a6 a5) a4) a3) a2) a1) ) := 
- 🏓 ursus_call_with_args ( LedgerableWithArgs := λ6 ) FLeXClient_Ф_preparePrice 
+ 🏓 ursus_call_with_args ( LedgerableWithArgs := λ6 ) FlexClient_Ф_preparePrice 
  ( SimpleLedgerableArg URValue {{ Λ "price" }} ( price ) ) 
  ( SimpleLedgerableArg URValue {{ Λ "min_amount" }} ( min_amount ) ) 
  ( SimpleLedgerableArg URValue {{ Λ "deals_limit" }} ( deals_limit ) ) 
@@ -537,18 +537,18 @@ Notation " 'error_code::message_sender_is_not_my_owner' " := (sInject error_code
  ( SimpleLedgerableArg URValue {{ Λ "tip3cfg" }} ( tip3cfg ) ) 
  ( SimpleLedgerableArg URValue {{ Λ "price_code" }} ( price_code ) ) 
  . 
- Notation " 'FLeXClient_Ф_preparePrice_ref_' '(' price min_amount deals_limit tip3_code tip3cfg price_code ')' " := 
+ Notation " 'FlexClient_Ф_preparePrice_ref_' '(' price min_amount deals_limit tip3_code tip3cfg price_code ')' " := 
  ( URResult ( FLeXClient_Ф_preparePrice_call 
  price min_amount deals_limit tip3_code tip3cfg price_code )) 
  (in custom URValue at level 0 , price custom URValue at level 0 
- , min_amount custom ULValue at level 0 
- , deals_limit custom ULValue at level 0 
- , tip3_code custom ULValue at level 0 
- , tip3cfg custom ULValue at level 0 
- , price_code custom ULValue at level 0 ) : ursus_scope . 
+ , min_amount custom URValue at level 0 
+ , deals_limit custom URValue at level 0 
+ , tip3_code custom URValue at level 0 
+ , tip3cfg custom URValue at level 0 
+ , price_code custom URValue at level 0 ) : ursus_scope . 
  
  Definition FLeXClient_Ф_deployPriceWithSell_call { a1 a2 a3 a4 a5 a6 a7 a8 a9 a10 }  ( price : URValue XInteger128 a1 ) ( amount : URValue XInteger128 a2 ) ( lend_finish_time : URValue XInteger32 a3 ) ( min_amount : URValue XInteger128 a4 ) ( deals_limit : URValue XInteger8 a5 ) ( tons_value : URValue XInteger128 a6 ) ( price_code : URValue TvmCell a7 ) ( my_tip3_addr : URValue addr_std_compact a8 ) ( receive_wallet : URValue addr_std_compact a9 ) ( tip3cfg : URValue Tip3Config a10 ) : LedgerT ( ControlResult XAddress true ) := 
- 🏓 ursus_call_with_args ( LedgerableWithArgs := λ10 ) FLeXClient_Ф_deployPriceWithSell 
+ 🏓 ursus_call_with_args ( LedgerableWithArgs := λ10 ) FlexClient_Ф_deployPriceWithSell 
  ( SimpleLedgerableArg URValue {{ Λ "price" }} ( price ) ) 
  ( SimpleLedgerableArg URValue {{ Λ "amount" }} ( amount ) ) 
  ( SimpleLedgerableArg URValue {{ Λ "lend_finish_time" }} ( lend_finish_time ) ) 
@@ -560,19 +560,19 @@ Notation " 'error_code::message_sender_is_not_my_owner' " := (sInject error_code
  ( SimpleLedgerableArg URValue {{ Λ "receive_wallet" }} ( receive_wallet ) ) 
  ( SimpleLedgerableArg URValue {{ Λ "tip3cfg" }} ( tip3cfg ) ) 
  . 
- Notation " 'FLeXClient_Ф_deployPriceWithSell_ref_' '(' price amount lend_finish_time min_amount deals_limit tons_value price_code my_tip3_addr receive_wallet tip3cfg ')' " := 
+ Notation " 'FlexClient_Ф_deployPriceWithSell_ref_' '(' price amount lend_finish_time min_amount deals_limit tons_value price_code my_tip3_addr receive_wallet tip3cfg ')' " := 
  ( URResult ( FLeXClient_Ф_deployPriceWithSell_call 
  price amount lend_finish_time min_amount deals_limit tons_value price_code my_tip3_addr receive_wallet tip3cfg )) 
  (in custom URValue at level 0 , price custom URValue at level 0 
- , amount custom ULValue at level 0 
- , lend_finish_time custom ULValue at level 0 
- , min_amount custom ULValue at level 0 
- , deals_limit custom ULValue at level 0 
- , tons_value custom ULValue at level 0 
- , price_code custom ULValue at level 0 
- , my_tip3_addr custom ULValue at level 0 
- , receive_wallet custom ULValue at level 0 
- , tip3cfg custom ULValue at level 0 ) : ursus_scope . 
+ , amount custom URValue at level 0 
+ , lend_finish_time custom URValue at level 0 
+ , min_amount custom URValue at level 0 
+ , deals_limit custom URValue at level 0 
+ , tons_value custom URValue at level 0 
+ , price_code custom URValue at level 0 
+ , my_tip3_addr custom URValue at level 0 
+ , receive_wallet custom URValue at level 0 
+ , tip3cfg custom URValue at level 0 ) : ursus_scope . 
  
  Definition FLeXClient_Ф_deployPriceWithBuy_call { a1 a2 a3 a4 a5 a6 a7 a8 a9 }  
 ( price : URValue XInteger128 a1 ) ( amount : URValue XInteger128 a2 ) 
@@ -580,7 +580,7 @@ Notation " 'error_code::message_sender_is_not_my_owner' " := (sInject error_code
 ( deals_limit : URValue XInteger8 a5 ) ( deploy_value : URValue XInteger128 a6 ) 
 ( price_code : URValue TvmCell a7 ) ( my_tip3_addr : URValue addr_std_compact a8 ) 
 ( tip3cfg : URValue Tip3Config a9 ) : LedgerT ( ControlResult XAddress true ) := 
- 🏓 ursus_call_with_args ( LedgerableWithArgs := λ9 ) FLeXClient_Ф_deployPriceWithBuy 
+ 🏓 ursus_call_with_args ( LedgerableWithArgs := λ9 ) FlexClient_Ф_deployPriceWithBuy 
  ( SimpleLedgerableArg URValue {{ Λ "price" }} ( price ) ) 
  ( SimpleLedgerableArg URValue {{ Λ "amount" }} ( amount ) ) 
  ( SimpleLedgerableArg URValue {{ Λ "order_finish_time" }} ( order_finish_time ) ) 
@@ -591,25 +591,25 @@ Notation " 'error_code::message_sender_is_not_my_owner' " := (sInject error_code
  ( SimpleLedgerableArg URValue {{ Λ "my_tip3_addr" }} ( my_tip3_addr ) ) 
  ( SimpleLedgerableArg URValue {{ Λ "tip3cfg" }} ( tip3cfg ) ) 
  . 
- Notation " 'FLeXClient_Ф_deployPriceWithBuy_ref_' '(' price amount order_finish_time min_amount deals_limit deploy_value price_code my_tip3_addr tip3cfg ')' " := 
+ Notation " 'FlexClient_Ф_deployPriceWithBuy_ref_' '(' price amount order_finish_time min_amount deals_limit deploy_value price_code my_tip3_addr tip3cfg ')' " := 
  ( URResult ( FLeXClient_Ф_deployPriceWithBuy_call 
  price amount order_finish_time min_amount deals_limit deploy_value price_code my_tip3_addr tip3cfg )) 
  (in custom URValue at level 0 , price custom URValue at level 0 
- , amount custom ULValue at level 0 
- , order_finish_time custom ULValue at level 0 
- , min_amount custom ULValue at level 0 
- , deals_limit custom ULValue at level 0 
- , deploy_value custom ULValue at level 0 
- , price_code custom ULValue at level 0 
- , my_tip3_addr custom ULValue at level 0 
- , tip3cfg custom ULValue at level 0 ) : ursus_scope . 
+ , amount custom URValue at level 0 
+ , order_finish_time custom URValue at level 0 
+ , min_amount custom URValue at level 0 
+ , deals_limit custom URValue at level 0 
+ , deploy_value custom URValue at level 0 
+ , price_code custom URValue at level 0 
+ , my_tip3_addr custom URValue at level 0 
+ , tip3cfg custom URValue at level 0 ) : ursus_scope . 
  
  Definition FLeXClient_Ф_cancelSellOrder_call { a1 a2 a3 a4 a5 a6 }  
 ( price : URValue XInteger128 a1 ) ( min_amount : URValue XInteger128 a2 ) 
 ( deals_limit : URValue XInteger8 a3 ) ( value : URValue XInteger128 a4 )
  ( price_code : URValue TvmCell a5 ) ( tip3cfg : URValue Tip3Config a6 ) 
 : LedgerT ( ControlResult PhantomType true ) := 
- 🏓 ursus_call_with_args ( LedgerableWithArgs := λ6 ) FLeXClient_Ф_cancelSellOrder 
+ 🏓 ursus_call_with_args ( LedgerableWithArgs := λ6 ) FlexClient_Ф_cancelSellOrder 
  ( SimpleLedgerableArg URValue {{ Λ "price" }} ( price ) ) 
  ( SimpleLedgerableArg URValue {{ Λ "min_amount" }} ( min_amount ) ) 
  ( SimpleLedgerableArg URValue {{ Λ "deals_limit" }} ( deals_limit ) ) 
@@ -617,21 +617,21 @@ Notation " 'error_code::message_sender_is_not_my_owner' " := (sInject error_code
  ( SimpleLedgerableArg URValue {{ Λ "price_code" }} ( price_code ) ) 
  ( SimpleLedgerableArg URValue {{ Λ "tip3cfg" }} ( tip3cfg ) ) 
  . 
- Notation " 'FLeXClient_Ф_cancelSellOrder_ref_' '(' price min_amount deals_limit value price_code tip3cfg ')' " := 
+ Notation " 'FlexClient_Ф_cancelSellOrder_ref_' '(' price min_amount deals_limit value price_code tip3cfg ')' " := 
  ( FuncallExpression ( FLeXClient_Ф_cancelSellOrder_call 
  price min_amount deals_limit value price_code tip3cfg )) 
- (in custom ULValue at level 0 , price custom ULValue at level 0 
- , min_amount custom ULValue at level 0 
- , deals_limit custom ULValue at level 0 
- , value custom ULValue at level 0 
- , price_code custom ULValue at level 0 
- , tip3cfg custom ULValue at level 0 ) : ursus_scope . 
+ (in custom ULValue at level 0 , price custom URValue at level 0 
+ , min_amount custom URValue at level 0 
+ , deals_limit custom URValue at level 0 
+ , value custom URValue at level 0 
+ , price_code custom URValue at level 0 
+ , tip3cfg custom URValue at level 0 ) : ursus_scope . 
  
  Definition FLeXClient_Ф_cancelBuyOrder_call { a1 a2 a3 a4 a5 a6 }  ( price : URValue XInteger128 a1 ) 
 ( min_amount : URValue XInteger128 a2 ) ( deals_limit : URValue XInteger8 a3 ) 
 ( value : URValue XInteger128 a4 ) ( price_code : URValue TvmCell a5 ) 
 ( tip3cfg : URValue Tip3Config a6 ) : LedgerT ( ControlResult PhantomType true ) := 
- 🏓 ursus_call_with_args ( LedgerableWithArgs := λ6 ) FLeXClient_Ф_cancelBuyOrder 
+ 🏓 ursus_call_with_args ( LedgerableWithArgs := λ6 ) FlexClient_Ф_cancelBuyOrder 
  ( SimpleLedgerableArg URValue {{ Λ "price" }} ( price ) ) 
  ( SimpleLedgerableArg URValue {{ Λ "min_amount" }} ( min_amount ) ) 
  ( SimpleLedgerableArg URValue {{ Λ "deals_limit" }} ( deals_limit ) ) 
@@ -639,22 +639,22 @@ Notation " 'error_code::message_sender_is_not_my_owner' " := (sInject error_code
  ( SimpleLedgerableArg URValue {{ Λ "price_code" }} ( price_code ) ) 
  ( SimpleLedgerableArg URValue {{ Λ "tip3cfg" }} ( tip3cfg ) ) 
  . 
- Notation " 'FLeXClient_Ф_cancelBuyOrder_ref_' '(' price min_amount deals_limit value price_code tip3cfg ')' " := 
+ Notation " 'FlexClient_Ф_cancelBuyOrder_ref_' '(' price min_amount deals_limit value price_code tip3cfg ')' " := 
  ( FuncallExpression ( FLeXClient_Ф_cancelBuyOrder_call 
  price min_amount deals_limit value price_code tip3cfg )) 
- (in custom ULValue at level 0 , price custom ULValue at level 0 
- , min_amount custom ULValue at level 0 
- , deals_limit custom ULValue at level 0 
- , value custom ULValue at level 0 
- , price_code custom ULValue at level 0 
- , tip3cfg custom ULValue at level 0 ) : ursus_scope . 
+ (in custom ULValue at level 0 , price custom URValue at level 0 
+ , min_amount custom URValue at level 0 
+ , deals_limit custom URValue at level 0 
+ , value custom URValue at level 0 
+ , price_code custom URValue at level 0 
+ , tip3cfg custom URValue at level 0 ) : ursus_scope . 
  
  Definition FLeXClient_Ф_preparePriceXchg_call { a1 a2 a3 a4 a5 a6 a7 }  ( price_num : URValue XInteger128 a1 )
  ( price_denum : URValue XInteger128 a2 ) ( min_amount : URValue XInteger128 a3 )
  ( deals_limit : URValue XInteger8 a4 ) ( major_tip3cfg : URValue Tip3Config a5 ) 
 ( minor_tip3cfg : URValue Tip3Config a6 ) ( price_code : URValue TvmCell a7 ) 
 : LedgerT ( ControlResult ( StateInit # XAddress # XInteger256 ) (orb (orb (orb (orb (orb (orb a7 a6) a5) a4) a3) a2) a1)) := 
- 🏓 ursus_call_with_args ( LedgerableWithArgs := λ7 ) FLeXClient_Ф_preparePriceXchg 
+ 🏓 ursus_call_with_args ( LedgerableWithArgs := λ7 ) FlexClient_Ф_preparePriceXchg 
  ( SimpleLedgerableArg URValue {{ Λ "price_num" }} ( price_num ) ) 
  ( SimpleLedgerableArg URValue {{ Λ "price_denum" }} ( price_denum ) ) 
  ( SimpleLedgerableArg URValue {{ Λ "min_amount" }} ( min_amount ) ) 
@@ -663,16 +663,16 @@ Notation " 'error_code::message_sender_is_not_my_owner' " := (sInject error_code
  ( SimpleLedgerableArg URValue {{ Λ "minor_tip3cfg" }} ( minor_tip3cfg ) ) 
  ( SimpleLedgerableArg URValue {{ Λ "price_code" }} ( price_code ) ) 
  . 
- Notation " 'FLeXClient_Ф_preparePriceXchg_ref_' '(' price_num price_denum min_amount deals_limit major_tip3cfg minor_tip3cfg price_code ')' " := 
+ Notation " 'FlexClient_Ф_preparePriceXchg_ref_' '(' price_num price_denum min_amount deals_limit major_tip3cfg minor_tip3cfg price_code ')' " := 
  ( URResult ( FLeXClient_Ф_preparePriceXchg_call 
  price_num price_denum min_amount deals_limit major_tip3cfg minor_tip3cfg price_code )) 
  (in custom URValue at level 0 , price_num custom URValue at level 0 
- , price_denum custom ULValue at level 0 
- , min_amount custom ULValue at level 0 
- , deals_limit custom ULValue at level 0 
- , major_tip3cfg custom ULValue at level 0 
- , minor_tip3cfg custom ULValue at level 0 
- , price_code custom ULValue at level 0 ) : ursus_scope . 
+ , price_denum custom URValue at level 0 
+ , min_amount custom URValue at level 0 
+ , deals_limit custom URValue at level 0 
+ , major_tip3cfg custom URValue at level 0 
+ , minor_tip3cfg custom URValue at level 0 
+ , price_code custom URValue at level 0 ) : ursus_scope . 
  
  Definition FLeXClient_Ф_cancelXchgOrder_call { a1 a2 a3 a4 a5 a6 a7 a8 a9 }  ( sell : URValue XBool a1 ) 
 ( price_num : URValue XInteger128 a2 ) ( price_denum : URValue XInteger128 a3 ) 
@@ -680,7 +680,7 @@ Notation " 'error_code::message_sender_is_not_my_owner' " := (sInject error_code
 ( value : URValue XInteger128 a6 ) ( xchg_price_code : URValue TvmCell a7 ) 
 ( major_tip3cfg : URValue Tip3Config a8 ) ( minor_tip3cfg : URValue Tip3Config a9 ) 
 : LedgerT ( ControlResult PhantomType true ) := 
- 🏓 ursus_call_with_args ( LedgerableWithArgs := λ9 ) FLeXClient_Ф_cancelXchgOrder 
+ 🏓 ursus_call_with_args ( LedgerableWithArgs := λ9 ) FlexClient_Ф_cancelXchgOrder 
  ( SimpleLedgerableArg URValue {{ Λ "sell" }} ( sell ) ) 
  ( SimpleLedgerableArg URValue {{ Λ "price_num" }} ( price_num ) ) 
  ( SimpleLedgerableArg URValue {{ Λ "price_denum" }} ( price_denum ) ) 
@@ -691,33 +691,33 @@ Notation " 'error_code::message_sender_is_not_my_owner' " := (sInject error_code
  ( SimpleLedgerableArg URValue {{ Λ "major_tip3cfg" }} ( major_tip3cfg ) ) 
  ( SimpleLedgerableArg URValue {{ Λ "minor_tip3cfg" }} ( minor_tip3cfg ) ) 
  . 
- Notation " 'FLeXClient_Ф_cancelXchgOrder_ref_' '(' sell price_num price_denum min_amount deals_limit value xchg_price_code major_tip3cfg minor_tip3cfg ')' " := 
+ Notation " 'FlexClient_Ф_cancelXchgOrder_ref_' '(' sell price_num price_denum min_amount deals_limit value xchg_price_code major_tip3cfg minor_tip3cfg ')' " := 
  ( FuncallExpression ( FLeXClient_Ф_cancelXchgOrder_call 
  sell price_num price_denum min_amount deals_limit value xchg_price_code major_tip3cfg minor_tip3cfg )) 
- (in custom ULValue at level 0 , sell custom ULValue at level 0 
- , price_num custom ULValue at level 0 
- , price_denum custom ULValue at level 0 
- , min_amount custom ULValue at level 0 
- , deals_limit custom ULValue at level 0 
- , value custom ULValue at level 0 
- , xchg_price_code custom ULValue at level 0 
- , major_tip3cfg custom ULValue at level 0 
- , minor_tip3cfg custom ULValue at level 0 ) : ursus_scope . 
+ (in custom ULValue at level 0 , sell custom URValue at level 0 
+ , price_num custom URValue at level 0 
+ , price_denum custom URValue at level 0 
+ , min_amount custom URValue at level 0 
+ , deals_limit custom URValue at level 0 
+ , value custom URValue at level 0 
+ , xchg_price_code custom URValue at level 0 
+ , major_tip3cfg custom URValue at level 0 
+ , minor_tip3cfg custom URValue at level 0 ) : ursus_scope . 
  
  Definition FLeXClient_Ф_transfer_call { a1 a2 a3 }  ( dest : URValue addr_std_compact a1 ) 
 ( value : URValue XInteger128 a2 ) ( bounce : URValue XBool a3 ) 
 : LedgerT ( ControlResult PhantomType true ) := 
- 🏓 ursus_call_with_args ( LedgerableWithArgs := λ3 ) FLeXClient_Ф_transfer 
+ 🏓 ursus_call_with_args ( LedgerableWithArgs := λ3 ) FlexClient_Ф_transfer 
  ( SimpleLedgerableArg URValue {{ Λ "dest" }} ( dest ) ) 
  ( SimpleLedgerableArg URValue {{ Λ "value" }} ( value ) ) 
  ( SimpleLedgerableArg URValue {{ Λ "bounce" }} ( bounce ) ) 
  . 
- Notation " 'FLeXClient_Ф_transfer_ref_' '(' dest value bounce ')' " := 
+ Notation " 'FlexClient_Ф_transfer_ref_' '(' dest value bounce ')' " := 
  ( FuncallExpression ( FLeXClient_Ф_transfer_call 
  dest value bounce )) 
- (in custom ULValue at level 0 , dest custom ULValue at level 0 
- , value custom ULValue at level 0 
- , bounce custom ULValue at level 0 ) : ursus_scope . 
+ (in custom ULValue at level 0 , dest custom URValue at level 0 
+ , value custom URValue at level 0 
+ , bounce custom URValue at level 0 ) : ursus_scope . 
  
  (* Definition FLeXClient_Ф_deployPriceXchg_call { a1 a2 a3 a4 a5 a6 a7 a8 a9 a10 a11 a12 a13 a14 } 
  ( sell : URValue XBool a1 ) ( price_num : URValue XInteger128 a2 ) 
@@ -729,7 +729,7 @@ Notation " 'error_code::message_sender_is_not_my_owner' " := (sInject error_code
 ( major_tip3cfg : URValue Tip3Config a13 ) ( minor_tip3cfg : URValue Tip3Config a14 ) 
 : LedgerT ( ControlResult XAddress  
 ( orb a14 ( orb a13 ( orb a12 ( orb a11 ( orb a10 ( orb a9 ( orb a8 ( orb a7 ( orb a6 ( orb a5 ( orb a4 ( orb a3 ( orb a2 a1 ) ) ) ) ) ) ) ) ) ) ) ) ) ) := 
- 🏓 ursus_call_with_args ( LedgerableWithArgs := λ14 ) FLeXClient_Ф_deployPriceXchg 
+ 🏓 ursus_call_with_args ( LedgerableWithArgs := λ14 ) FlexClient_Ф_deployPriceXchg 
  ( SimpleLedgerableArg URValue {{ Λ "sell" }} ( sell ) ) 
  ( SimpleLedgerableArg URValue {{ Λ "price_num" }} ( price_num ) ) 
  ( SimpleLedgerableArg URValue {{ Λ "price_denum" }} ( price_denum ) ) 
@@ -745,30 +745,30 @@ Notation " 'error_code::message_sender_is_not_my_owner' " := (sInject error_code
  ( SimpleLedgerableArg URValue {{ Λ "major_tip3cfg" }} ( major_tip3cfg ) ) 
  ( SimpleLedgerableArg URValue {{ Λ "minor_tip3cfg" }} ( minor_tip3cfg ) ) 
  . 
- Notation " 'FLeXClient_Ф_deployPriceXchg_ref_' '(' sell price_num price_denum amount lend_amount lend_finish_time min_amount deals_limit tons_value xchg_price_code my_tip3_addr receive_wallet major_tip3cfg minor_tip3cfg ')' " := 
+ Notation " 'FlexClient_Ф_deployPriceXchg_ref_' '(' sell price_num price_denum amount lend_amount lend_finish_time min_amount deals_limit tons_value xchg_price_code my_tip3_addr receive_wallet major_tip3cfg minor_tip3cfg ')' " := 
  ( URResult ( FLeXClient_Ф_deployPriceXchg_call 
  sell price_num price_denum amount lend_amount lend_finish_time min_amount deals_limit tons_value xchg_price_code my_tip3_addr receive_wallet major_tip3cfg minor_tip3cfg )) 
  (in custom URValue at level 0 , sell custom URValue at level 0 
- , price_num custom ULValue at level 0 
- , price_denum custom ULValue at level 0 
- , amount custom ULValue at level 0 
- , lend_amount custom ULValue at level 0 
- , lend_finish_time custom ULValue at level 0 
- , min_amount custom ULValue at level 0 
- , deals_limit custom ULValue at level 0 
- , tons_value custom ULValue at level 0 
- , xchg_price_code custom ULValue at level 0 
- , my_tip3_addr custom ULValue at level 0 
- , receive_wallet custom ULValue at level 0 
- , major_tip3cfg custom ULValue at level 0 
- , minor_tip3cfg custom ULValue at level 0 ) : ursus_scope . 
+ , price_num custom URValue at level 0 
+ , price_denum custom URValue at level 0 
+ , amount custom URValue at level 0 
+ , lend_amount custom URValue at level 0 
+ , lend_finish_time custom URValue at level 0 
+ , min_amount custom URValue at level 0 
+ , deals_limit custom URValue at level 0 
+ , tons_value custom URValue at level 0 
+ , xchg_price_code custom URValue at level 0 
+ , my_tip3_addr custom URValue at level 0 
+ , receive_wallet custom URValue at level 0 
+ , major_tip3cfg custom URValue at level 0 
+ , minor_tip3cfg custom URValue at level 0 ) : ursus_scope . 
   *)
  Definition FLeXClient_Ф_deployWrapperWithWallet_call { a1 a2 a3 a4 a5 a6 } 
  ( wrapper_pubkey : URValue XInteger256 a1 ) ( wrapper_deploy_value : URValue XInteger128 a2 )
  ( wrapper_keep_balance : URValue XInteger128 a3 ) ( ext_wallet_balance : URValue XInteger128 a4 ) 
 ( set_internal_wallet_value : URValue XInteger128 a5 ) ( tip3cfg : URValue Tip3Config a6 ) 
 : LedgerT ( ControlResult XAddress true  ) := 
- 🏓 ursus_call_with_args ( LedgerableWithArgs := λ6 ) FLeXClient_Ф_deployWrapperWithWallet 
+ 🏓 ursus_call_with_args ( LedgerableWithArgs := λ6 ) FlexClient_Ф_deployWrapperWithWallet 
  ( SimpleLedgerableArg URValue {{ Λ "wrapper_pubkey" }} ( wrapper_pubkey ) ) 
  ( SimpleLedgerableArg URValue {{ Λ "wrapper_deploy_value" }} ( wrapper_deploy_value ) ) 
  ( SimpleLedgerableArg URValue {{ Λ "wrapper_keep_balance" }} ( wrapper_keep_balance ) ) 
@@ -776,84 +776,84 @@ Notation " 'error_code::message_sender_is_not_my_owner' " := (sInject error_code
  ( SimpleLedgerableArg URValue {{ Λ "set_internal_wallet_value" }} ( set_internal_wallet_value ) ) 
  ( SimpleLedgerableArg URValue {{ Λ "tip3cfg" }} ( tip3cfg ) ) 
  . 
- Notation " 'FLeXClient_Ф_deployWrapperWithWallet_ref_' '(' wrapper_pubkey wrapper_deploy_value wrapper_keep_balance ext_wallet_balance set_internal_wallet_value tip3cfg ')' " := 
+ Notation " 'FlexClient_Ф_deployWrapperWithWallet_ref_' '(' wrapper_pubkey wrapper_deploy_value wrapper_keep_balance ext_wallet_balance set_internal_wallet_value tip3cfg ')' " := 
  ( URResult ( FLeXClient_Ф_deployWrapperWithWallet_call 
  wrapper_pubkey wrapper_deploy_value wrapper_keep_balance ext_wallet_balance set_internal_wallet_value tip3cfg )) 
  (in custom URValue at level 0 , wrapper_pubkey custom URValue at level 0 
- , wrapper_deploy_value custom ULValue at level 0 
- , wrapper_keep_balance custom ULValue at level 0 
- , ext_wallet_balance custom ULValue at level 0 
- , set_internal_wallet_value custom ULValue at level 0 
- , tip3cfg custom ULValue at level 0 ) : ursus_scope . 
+ , wrapper_deploy_value custom URValue at level 0 
+ , wrapper_keep_balance custom URValue at level 0 
+ , ext_wallet_balance custom URValue at level 0 
+ , set_internal_wallet_value custom URValue at level 0 
+ , tip3cfg custom URValue at level 0 ) : ursus_scope . 
  
  Definition FLeXClient_Ф_deployEmptyFlexWallet_call { a1 a2 a3 }  ( pubkey : URValue XInteger256 a1 ) 
 ( tons_to_wallet : URValue XInteger128 a2 ) ( tip3cfg : URValue Tip3Config a3 ) 
 : LedgerT ( ControlResult XAddress true  ) := 
- 🏓 ursus_call_with_args ( LedgerableWithArgs := λ3 ) FLeXClient_Ф_deployEmptyFlexWallet 
+ 🏓 ursus_call_with_args ( LedgerableWithArgs := λ3 ) FlexClient_Ф_deployEmptyFlexWallet 
  ( SimpleLedgerableArg URValue {{ Λ "pubkey" }} ( pubkey ) ) 
  ( SimpleLedgerableArg URValue {{ Λ "tons_to_wallet" }} ( tons_to_wallet ) ) 
  ( SimpleLedgerableArg URValue {{ Λ "tip3cfg" }} ( tip3cfg ) ) 
  . 
- Notation " 'FLeXClient_Ф_deployEmptyFlexWallet_ref_' '(' pubkey tons_to_wallet tip3cfg ')' " := 
+ Notation " 'FlexClient_Ф_deployEmptyFlexWallet_ref_' '(' pubkey tons_to_wallet tip3cfg ')' " := 
  ( URResult ( FLeXClient_Ф_deployEmptyFlexWallet_call 
  pubkey tons_to_wallet tip3cfg )) 
  (in custom URValue at level 0 , pubkey custom URValue at level 0 
- , tons_to_wallet custom ULValue at level 0 
- , tip3cfg custom ULValue at level 0 ) : ursus_scope . 
+ , tons_to_wallet custom URValue at level 0 
+ , tip3cfg custom URValue at level 0 ) : ursus_scope . 
  
  Definition FLeXClient_Ф_burnWallet_call { a1 a2 a3 a4 }  ( tons_value : URValue XInteger128 a1 ) 
 ( out_pubkey : URValue XInteger256 a2 ) ( out_internal_owner : URValue addr_std_compact a3 ) 
 ( my_tip3_addr : URValue addr_std_compact a4 ) : LedgerT ( ControlResult PhantomType true ) := 
- 🏓 ursus_call_with_args ( LedgerableWithArgs := λ4 ) FLeXClient_Ф_burnWallet 
+ 🏓 ursus_call_with_args ( LedgerableWithArgs := λ4 ) FlexClient_Ф_burnWallet 
  ( SimpleLedgerableArg URValue {{ Λ "tons_value" }} ( tons_value ) ) 
  ( SimpleLedgerableArg URValue {{ Λ "out_pubkey" }} ( out_pubkey ) ) 
  ( SimpleLedgerableArg URValue {{ Λ "out_internal_owner" }} ( out_internal_owner ) ) 
  ( SimpleLedgerableArg URValue {{ Λ "my_tip3_addr" }} ( my_tip3_addr ) ) 
  . 
- Notation " 'FLeXClient_Ф_burnWallet_ref_' '(' tons_value out_pubkey out_internal_owner my_tip3_addr ')' " := 
+ Notation " 'FlexClient_Ф_burnWallet_ref_' '(' tons_value out_pubkey out_internal_owner my_tip3_addr ')' " := 
  ( FuncallExpression ( FLeXClient_Ф_burnWallet_call 
  tons_value out_pubkey out_internal_owner my_tip3_addr )) 
- (in custom ULValue at level 0 , tons_value custom ULValue at level 0 
- , out_pubkey custom ULValue at level 0 
- , out_internal_owner custom ULValue at level 0 
- , my_tip3_addr custom ULValue at level 0 ) : ursus_scope . 
+ (in custom ULValue at level 0 , tons_value custom URValue at level 0 
+ , out_pubkey custom URValue at level 0 
+ , out_internal_owner custom URValue at level 0 
+ , my_tip3_addr custom URValue at level 0 ) : ursus_scope . 
  
  Definition FLeXClient_Ф_getOwner_call  : LedgerT ( ControlResult XInteger256 false ) := 
- 🏓 ursus_call_with_args ( LedgerableWithArgs := λ0 ) FLeXClient_Ф_getOwner 
+ 🏓 ursus_call_with_args ( LedgerableWithArgs := λ0 ) FlexClient_Ф_getOwner 
  . 
- Notation " 'FLeXClient_Ф_getOwner_ref_' '(' ')' " := 
+ Notation " 'FlexClient_Ф_getOwner_ref_' '(' ')' " := 
  ( URResult ( FLeXClient_Ф_getOwner_call 
  )) 
  (in custom URValue at level 0 ) : ursus_scope . 
  
  Definition FLeXClient_Ф_getFlex_call  : LedgerT ( ControlResult XAddress false ) := 
- 🏓 ursus_call_with_args ( LedgerableWithArgs := λ0 ) FLeXClient_Ф_getFlex 
+ 🏓 ursus_call_with_args ( LedgerableWithArgs := λ0 ) FlexClient_Ф_getFlex 
  . 
- Notation " 'FLeXClient_Ф_getFlex_ref_' '(' ')' " := 
+ Notation " 'FlexClient_Ф_getFlex_ref_' '(' ')' " := 
  ( URResult ( FLeXClient_Ф_getFlex_call 
  )) 
  (in custom URValue at level 0 ) : ursus_scope . 
  
  Definition FLeXClient_Ф_hasExtWalletCode_call  : LedgerT ( ControlResult XBool false ) := 
- 🏓 ursus_call_with_args ( LedgerableWithArgs := λ0 ) FLeXClient_Ф_hasExtWalletCode 
+ 🏓 ursus_call_with_args ( LedgerableWithArgs := λ0 ) FlexClient_Ф_hasExtWalletCode 
  . 
- Notation " 'FLeXClient_Ф_hasExtWalletCode_ref_' '(' ')' " := 
+ Notation " 'FlexClient_Ф_hasExtWalletCode_ref_' '(' ')' " := 
  ( URResult ( FLeXClient_Ф_hasExtWalletCode_call 
  )) 
  (in custom URValue at level 0 ) : ursus_scope . 
  
  Definition FLeXClient_Ф_hasFlexWalletCode_call  : LedgerT ( ControlResult XBool false ) := 
- 🏓 ursus_call_with_args ( LedgerableWithArgs := λ0 ) FLeXClient_Ф_hasFlexWalletCode 
+ 🏓 ursus_call_with_args ( LedgerableWithArgs := λ0 ) FlexClient_Ф_hasFlexWalletCode 
  . 
- Notation " 'FLeXClient_Ф_hasFlexWalletCode_ref_' '(' ')' " := 
+ Notation " 'FlexClient_Ф_hasFlexWalletCode_ref_' '(' ')' " := 
  ( URResult ( FLeXClient_Ф_hasFlexWalletCode_call 
  )) 
  (in custom URValue at level 0 ) : ursus_scope . 
  
  Definition FLeXClient_Ф_hasFlexWrapperCode_call  : LedgerT ( ControlResult XBool false ) := 
- 🏓 ursus_call_with_args ( LedgerableWithArgs := λ0 ) FLeXClient_Ф_hasFlexWrapperCode 
+ 🏓 ursus_call_with_args ( LedgerableWithArgs := λ0 ) FlexClient_Ф_hasFlexWrapperCode 
  . 
- Notation " 'FLeXClient_Ф_hasFlexWrapperCode_ref_' '(' ')' " := 
+ Notation " 'FlexClient_Ф_hasFlexWrapperCode_ref_' '(' ')' " := 
  ( URResult ( FLeXClient_Ф_hasFlexWrapperCode_call 
  )) 
  (in custom URValue at level 0 ) : ursus_scope . 
@@ -861,23 +861,23 @@ Notation " 'error_code::message_sender_is_not_my_owner' " := (sInject error_code
  Definition FLeXClient_Ф_getPayloadForDeployInternalWallet_call { a1 a2 a3 } 
  ( owner_pubkey : URValue XInteger256 a1 ) ( owner_addr : URValue addr_std_compact a2 )
  ( tons : URValue XInteger128 a3 ) : LedgerT ( ControlResult TvmCell (orb (orb a3 a2) a1) ) := 
- 🏓 ursus_call_with_args ( LedgerableWithArgs := λ3 ) FLeXClient_Ф_getPayloadForDeployInternalWallet 
+ 🏓 ursus_call_with_args ( LedgerableWithArgs := λ3 ) FlexClient_Ф_getPayloadForDeployInternalWallet 
  ( SimpleLedgerableArg URValue {{ Λ "owner_pubkey" }} ( owner_pubkey ) ) 
  ( SimpleLedgerableArg URValue {{ Λ "owner_addr" }} ( owner_addr ) ) 
  ( SimpleLedgerableArg URValue {{ Λ "tons" }} ( tons ) ) 
  . 
- Notation " 'FLeXClient_Ф_getPayloadForDeployInternalWallet_ref_' '(' owner_pubkey owner_addr tons ')' " := 
+ Notation " 'FlexClient_Ф_getPayloadForDeployInternalWallet_ref_' '(' owner_pubkey owner_addr tons ')' " := 
  ( URResult ( FLeXClient_Ф_getPayloadForDeployInternalWallet_call 
  owner_pubkey owner_addr tons )) 
  (in custom URValue at level 0 , owner_pubkey custom URValue at level 0 
- , owner_addr custom ULValue at level 0 
- , tons custom ULValue at level 0 ) : ursus_scope . 
+ , owner_addr custom URValue at level 0 
+ , tons custom URValue at level 0 ) : ursus_scope . 
 
  Definition FLeXClient_Ф__fallback_call { a1 }  ( x : URValue TvmCell a1 ) : LedgerT ( ControlResult XInteger a1 ) := 
- 🏓 ursus_call_with_args ( LedgerableWithArgs := λ1 ) FLeXClient_Ф__fallback 
+ 🏓 ursus_call_with_args ( LedgerableWithArgs := λ1 ) FlexClient_Ф__fallback 
  ( SimpleLedgerableArg URValue {{ Λ "x" }} ( x ) ) 
  . 
- Notation " 'FLeXClient_Ф__fallback_ref_' '(' cell ')' " := 
+ Notation " 'FlexClient_Ф__fallback_ref_' '(' cell ')' " := 
  ( URResult ( FLeXClient_Ф__fallback_call 
  cell )) 
  (in custom URValue at level 0 , cell custom URValue at level 0 ) : ursus_scope . 
