src/FLeXFuncs.v
@@ -65,78 +65,78 @@ Definition Flex_Ф_constructor ( deployer_pubkey : XInteger256 ) ( transfer_tip3
  	 	 refine {{ send_notify : ( XInteger128 ) @ "send_notify" ; { _ } }} . 
  	 	 refine {{ deals_limit : ( XInteger8 ) @ "deals_limit" ; { _ } }} . 
  	 	 refine {{ notify_addr : ( XAddress ) @ "notify_addr" ; { _ } }} . 
- 	 	 refine {{ FLeX.deployer_pubkey_ := !{ deployer_pubkey } ; { _ } }} . 
- 	 	 refine {{ FLeX.deals_limit_ := !{ deals_limit } ; { _ } }} . 
- 	 	 refine {{ FLeX.notify_addr_ := !{ notify_addr } ; { _ } }} . 
- 	 	 refine {{ FLeX.tons_cfg_ := {} (* { !{ transfer_tip3 } , !{ return_ownership } , !{ trading_pair_deploy } , !{ order_answer } , !{ process_queue } , !{ send_notify } } *) }} . 
+ 	 	 refine {{ Flex.deployer_pubkey_ := !{ deployer_pubkey } ; { _ } }} . 
+ 	 	 refine {{ Flex.deals_limit_ := !{ deals_limit } ; { _ } }} . 
+ 	 	 refine {{ Flex.notify_addr_ := !{ notify_addr } ; { _ } }} . 
+ 	 	 refine {{ Flex.tons_cfg_ := {} (* { !{ transfer_tip3 } , !{ return_ownership } , !{ trading_pair_deploy } , !{ order_answer } , !{ process_queue } , !{ send_notify } } *) }} . 
  Defined . 
  
  
  Definition Flex_Ф_setPairCode ( code : TvmCell ) : UExpression PhantomType true . 
  	 	 refine {{ code : ( TvmCell ) @ "code" ; { _ } }} . 
- 	 	 refine {{ require_ ( ( ~ TRUE (* FLeX.pair_code_ *) ) , error_code::cant_override_code ) ; { _ } }} . 
- 	 	 refine {{ require_ ( ( msg.pubkey () == FLeX.deployer_pubkey_ ) , error_code::sender_is_not_deployer ) ; { _ } }} . 
+ 	 	 refine {{ require_ ( ( ~ TRUE (* Flex.pair_code_ *) ) , error_code::cant_override_code ) ; { _ } }} . 
+ 	 	 refine {{ require_ ( ( msg.pubkey () == Flex.deployer_pubkey_ ) , error_code::sender_is_not_deployer ) ; { _ } }} . 
 (*  	 	 refine {{ tvm.accept () ; { _ } }} .  *)
  	 	 refine {{ require_ ( (* ( code.ctos ( ) . srefs ( ) *) 1 == 1 (* 2 *) , error_code::unexpected_refs_count_in_code ) ; { _ } }} . 
- 	 	 refine {{ FLeX.pair_code_ := {} (* builder ( ) . stslice ( code ^^ TvmCell:ctos ( ) ) . stref ( build ( Address { tvm_myaddr ( ) } ) . endc ( ) ) . endc ( )  *) }} . 
+ 	 	 refine {{ Flex.pair_code_ := {} (* builder ( ) . stslice ( code ^^ TvmCell:ctos ( ) ) . stref ( build ( Address { tvm_myaddr ( ) } ) . endc ( ) ) . endc ( )  *) }} . 
  Defined . 
  
  
  Definition Flex_Ф_setXchgPairCode ( code : TvmCell ) : UExpression PhantomType true . 
  	 	 refine {{ code : ( TvmCell ) @ "code" ; { _ } }} . 
- 	 	 refine {{ require_ ( TRUE (* ~ FLeX.xchg_pair_code_ *) , error_code::cant_override_code ) ; { _ } }} . 
- 	 	 refine {{ require_ ( ( msg.pubkey () == FLeX.deployer_pubkey_ ) , error_code::sender_is_not_deployer ) ; { _ } }} . 
+ 	 	 refine {{ require_ ( TRUE (* ~ Flex.xchg_pair_code_ *) , error_code::cant_override_code ) ; { _ } }} . 
+ 	 	 refine {{ require_ ( ( msg.pubkey () == Flex.deployer_pubkey_ ) , error_code::sender_is_not_deployer ) ; { _ } }} . 
 (*  	 	 refine {{ tvm.accept () ; { _ } }} .  *)
  	 	 refine {{ require_ ( (* ( code.ctos ( ) . srefs ( ) == 2 )  *) 1 == 1 , error_code::unexpected_refs_count_in_code ) ; { _ } }} . 
- 	 	 refine {{ FLeX.xchg_pair_code_ := {} (* builder ( ) . stslice ( code.ctos ( ) ) . stref ( build ( Address { tvm_myaddr ( ) } ) . endc ( ) ) . endc ( ) *)  }} . 
+ 	 	 refine {{ Flex.xchg_pair_code_ := {} (* builder ( ) . stslice ( code.ctos ( ) ) . stref ( build ( Address { tvm_myaddr ( ) } ) . endc ( ) ) . endc ( ) *)  }} . 
  Defined . 
  
  
  Definition Flex_Ф_setPriceCode ( code : TvmCell ) : UExpression PhantomType true . 
  	 	 refine {{ code : ( TvmCell ) @ "code" ; { _ } }} . 
- 	 	 refine {{ require_ ( ( ~ TRUE (* FLeX.price_code_ *) ) , error_code::cant_override_code ) ; { _ } }} . 
- 	 	 refine {{ require_ ( ( msg.pubkey () == FLeX.deployer_pubkey_ ) , error_code::sender_is_not_deployer ) ; { _ } }} . 
+ 	 	 refine {{ require_ ( ( ~ TRUE (* Flex.price_code_ *) ) , error_code::cant_override_code ) ; { _ } }} . 
+ 	 	 refine {{ require_ ( ( msg.pubkey () == Flex.deployer_pubkey_ ) , error_code::sender_is_not_deployer ) ; { _ } }} . 
 (*  	 	 refine {{ tvm.accept () ; { _ } }} .  *)
- 	 	 refine {{ FLeX.price_code_ ->set !{ code }  }} . 
+ 	 	 refine {{ Flex.price_code_ ->set !{ code }  }} . 
  Defined . 
  
  
  Definition Flex_Ф_setXchgPriceCode ( code : TvmCell ) : UExpression PhantomType true . 
  	 	 refine {{ code : ( TvmCell ) @ "code" ; { _ } }} . 
- 	 	 refine {{ require_ ( ( ~ TRUE (* FLeX.xchg_price_code_ *) ) , error_code::cant_override_code ) ; { _ } }} . 
- 	 	 refine {{ require_ ( ( msg.pubkey () == FLeX.deployer_pubkey_ ) , error_code::sender_is_not_deployer ) ; { _ } }} . 
+ 	 	 refine {{ require_ ( ( ~ TRUE (* Flex.xchg_price_code_ *) ) , error_code::cant_override_code ) ; { _ } }} . 
+ 	 	 refine {{ require_ ( ( msg.pubkey () == Flex.deployer_pubkey_ ) , error_code::sender_is_not_deployer ) ; { _ } }} . 
 (*  	 	 refine {{ tvm.accept () ; { _ } }} .  *)
- 	 	 refine {{ FLeX.xchg_price_code_ ->set !{ code } }} . 
+ 	 	 refine {{ Flex.xchg_price_code_ ->set !{ code } }} . 
  Defined . 
  
  
  Definition Flex_Ф_isFullyInitialized : UExpression XBool false . 
- 	 	 refine {{ return_ {} (* FLeX.pair_code_ && FLeX.price_code_ && FLeX.xchg_pair_code_ && FLeX.xchg_price_code_ *) }} . 
+ 	 	 refine {{ return_ {} (* Flex.pair_code_ && Flex.price_code_ && Flex.xchg_pair_code_ && Flex.xchg_price_code_ *) }} . 
  Defined . 
  
  
  
  Definition Flex_Ф_getTonsCfg : UExpression TonsConfig false . 
- 	 	 refine {{ return_ FLeX.tons_cfg_ }} . 
+ 	 	 refine {{ return_ Flex.tons_cfg_ }} . 
  Defined . 
  
  
  
  Definition Flex_Ф_getTradingPairCode : UExpression TvmCell false (* true *) . 
- 	 	 refine {{ return_ {} (* (FLeX.pair_code_ ->get) *) }} . 
+ 	 	 refine {{ return_ {} (* (Flex.pair_code_ ->get) *) }} . 
  Defined . 
  
  
  
  Definition Flex_Ф_getXchgPairCode : UExpression TvmCell false . 
- 	 	 refine {{ return_ {} (* (FLeX.xchg_pair_code_ ->get) *) }} . 
+ 	 	 refine {{ return_ {} (* (Flex.xchg_pair_code_ ->get) *) }} . 
  Defined . 
  
  
  
  Definition Flex_Ф_getSellPriceCode ( tip3_addr : XAddress ) : UExpression TvmCell true . 
  	 	 refine {{ tip3_addr : ( XAddress ) @ "tip3_addr" ; { _ } }} . 
- 	 	 refine {{ require_ ( ( (* FLeX.price_code_ - > ctos ( ) . srefs ( ) == 2 *) 1 == 1 ) , error_code::unexpected_refs_count_in_code ) ; { _ } }} . 
+ 	 	 refine {{ require_ ( ( (* Flex.price_code_ - > ctos ( ) . srefs ( ) == 2 *) 1 == 1 ) , error_code::unexpected_refs_count_in_code ) ; { _ } }} . 
  	 	 refine {{ (* new *) salt : ( TvmCell ) @"salt" ; { _ } }} . 
  	 	 refine {{ { salt } := {} (* builder ( ) . stslice ( tvm_myaddr ( ) ) . stslice ( tip3_addr ^^ XAddress:sl ( ) ) . endc ( ) *) ; { _ } }} . 
  	 	 refine {{ return_ {} (* builder ( ) . stslice ( price_code_ - > ctos ( ) ) . stref ( !{ salt } ) . endc ( ) *) }} . 
@@ -147,7 +147,7 @@ Definition Flex_Ф_constructor ( deployer_pubkey : XInteger256 ) ( transfer_tip3
  Definition Flex_Ф_getXchgPriceCode ( tip3_addr1 : XAddress ) ( tip3_addr2 : XAddress ) : UExpression TvmCell true . 
  	 	 refine {{ tip3_addr1 : ( XAddress ) @ "tip3_addr1" ; { _ } }} . 
  	 	 refine {{ tip3_addr2 : ( XAddress ) @ "tip3_addr2" ; { _ } }} . 
- 	 	 refine {{ require_ ( ( (* FLeX.price_code_ - > ctos ( ) . srefs ( ) == 2 *) 1 == 1 ) , error_code::unexpected_refs_count_in_code ) ; { _ } }} . 
+ 	 	 refine {{ require_ ( ( (* Flex.price_code_ - > ctos ( ) . srefs ( ) == 2 *) 1 == 1 ) , error_code::unexpected_refs_count_in_code ) ; { _ } }} . 
  	 	 refine {{ (* new *) keys : ( XAddress * XAddress ) @ "keys" ; { _ } }} . 
  	 	 refine {{ { keys } := {} (* [ !{ tip3_addr1 } , !{ tip3_addr2 } ] *) ; { _ } }} . 
  	 	 refine {{ return_ {} (* builder ( ) . stslice ( xchg_price_code_ - > ctos ( ) ) . stref ( build ( !{ keys } ) . endc ( ) ) . endc ( )  *) }} . 
@@ -162,7 +162,7 @@ Definition Flex_Ф_constructor ( deployer_pubkey : XInteger256 ) ( transfer_tip3
  	 	 refine {{ (* new *) pair_data : ( TradingPair ) @ "pair_data" ; { _ } }} . 
  	 	 refine {{ { pair_data } := {} (* NEW { . flex_addr_ = myaddr , . tip3_root_ = tip3_root , . min_amount_ = uint128 ( 0 ) } *) ; { _ } }} . 
  	 	 refine {{ (* new *) std_addr : ( StateInit * XInteger256 ) @ "std_addr" ; { _ } }} . 
- 	 	 refine {{ { std_addr } := {} (* prepare_trading_pair_state_init_and_addr ( !{ pair_data } , FLeX.pair_code_ ->get ) ->second *) ; { _ } }} . 
+ 	 	 refine {{ { std_addr } := {} (* prepare_trading_pair_state_init_and_addr ( !{ pair_data } , Flex.pair_code_ ->get ) ->second *) ; { _ } }} . 
  	 	 refine {{ (* new *) workchain_id : ( auto ) @ "workchain_id" ; { _ } }} . 
  	 	 refine {{ { workchain_id } := {} (* Std :: get < addr_std > ( myaddr ^^ address:val ( ) ) . workchain_id *) ; { _ } }} . 
  	 	 refine {{ return_ {} (* Address :: make_std ( !{ workchain_id } , !{ std_addr } ) *) }} . 
@@ -178,7 +178,7 @@ Definition Flex_Ф_constructor ( deployer_pubkey : XInteger256 ) ( transfer_tip3
  	 	 refine {{ (* new *) pair_data : ( XchgPair ) @ "pair_data" ; { _ } }} . 
  	 	 refine {{ { pair_data } := {} (* NEW { . flex_addr_ = myaddr , . tip3_major_root_ = tip3_major_root , . tip3_minor_root_ = tip3_minor_root , . min_amount_ = uint128 ( 0 ) } *) ; { _ } }} . 
  	 	 refine {{ (* new *) std_addr : ( auto ) @ "std_addr" ; { _ } }} . 
- 	 	 refine {{ { std_addr } := {} (* prepare_xchg_pair_state_init_and_addr ( !{ pair_data } , FLeX.xchg_pair_code_ ->get ) ->second *) ; { _ } }} . 
+ 	 	 refine {{ { std_addr } := {} (* prepare_xchg_pair_state_init_and_addr ( !{ pair_data } , Flex.xchg_pair_code_ ->get ) ->second *) ; { _ } }} . 
  	 	 refine {{ (* new *) workchain_id : ( auto ) @ "workchain_id" ; { _ } }} . 
  	 	 refine {{ { workchain_id } := {} (* Std :: get < addr_std > ( myaddr ^^ address:val ( ) ) . workchain_id *) ; { _ } }} . 
  	 	 refine {{ return_ {} (* Address :: make_std ( !{ workchain_id } , !{ std_addr } ) *) }} . 
@@ -187,13 +187,13 @@ Definition Flex_Ф_constructor ( deployer_pubkey : XInteger256 ) ( transfer_tip3
  
  
  Definition Flex_Ф_getDealsLimit : UExpression XInteger8 false . 
- 	 	 refine {{ return_ FLeX.deals_limit_ }} . 
+ 	 	 refine {{ return_ Flex.deals_limit_ }} . 
  Defined . 
  
  
  
  Definition Flex_Ф_getNotifyAddr : UExpression XAddress false . 
- 	 	 refine {{ return_ FLeX.notify_addr_ }} . 
+ 	 	 refine {{ return_ Flex.notify_addr_ }} . 
  Defined . 
  
  
