src/FLeXClientSpecs.v
@@ -19,32 +19,32 @@ Module Type specFLeXClientSig.
 
 
 
-Parameter FLeXClient_Ф_constructor : XInteger256 -> TvmCell -> TvmCell -> UExpression PhantomType true . 
- Parameter FLeXClient_Ф_setFlexCfg : TonsConfig -> addr_std_compact -> addr_std_compact -> UExpression PhantomType true . 
- Parameter FLeXClient_Ф_setExtWalletCode : TvmCell -> UExpression PhantomType true . 
- Parameter FLeXClient_Ф_setFlexWalletCode : TvmCell -> UExpression PhantomType true . 
- Parameter FLeXClient_Ф_setFlexWrapperCode : TvmCell -> UExpression PhantomType true . 
- Parameter FLeXClient_Ф_deployTradingPair : addr_std_compact -> XInteger128 -> XInteger128 -> XInteger128 -> UExpression XAddress true . 
- Parameter FLeXClient_Ф_deployXchgPair : addr_std_compact -> addr_std_compact -> XInteger128 -> XInteger128 -> XInteger128 -> UExpression XAddress true . 
-(*  Parameter FLeXClient_Ф_preparePrice : XInteger128 -> XInteger128 -> XInteger8 -> TvmCell -> Tip3Config -> TvmCell -> UExpression ( StateInit # XAddress # XInteger256 )%type false .  *)
- Parameter FLeXClient_Ф_deployPriceWithSell : XInteger128 -> XInteger128 -> XInteger32 -> XInteger128 -> XInteger8 -> XInteger128 -> TvmCell -> addr_std_compact -> addr_std_compact -> Tip3Config -> UExpression XAddress true . 
- Parameter FLeXClient_Ф_deployPriceWithBuy : XInteger128 -> XInteger128 -> XInteger32 -> XInteger128 -> XInteger8 -> XInteger128 -> TvmCell -> addr_std_compact -> Tip3Config -> UExpression XAddress true . 
- Parameter FLeXClient_Ф_cancelSellOrder : XInteger128 -> XInteger128 -> XInteger8 -> XInteger128 -> TvmCell -> Tip3Config -> UExpression PhantomType true . 
- Parameter FLeXClient_Ф_cancelBuyOrder : XInteger128 -> XInteger128 -> XInteger8 -> XInteger128 -> TvmCell -> Tip3Config -> UExpression PhantomType true . 
-(*  Parameter FLeXClient_Ф_preparePriceXchg : XInteger128 -> XInteger128 -> XInteger128 -> XInteger8 -> Tip3Config -> Tip3Config -> TvmCell -> UExpression ( StateInit # XAddress # XInteger256 )%type false .  *)
- Parameter FLeXClient_Ф_cancelXchgOrder : XBool -> XInteger128 -> XInteger128 -> XInteger128 -> XInteger8 -> XInteger128 -> TvmCell -> Tip3Config -> Tip3Config -> UExpression PhantomType true . 
- Parameter FLeXClient_Ф_transfer : addr_std_compact -> XInteger128 -> XBool -> UExpression PhantomType true . 
- Parameter FLeXClient_Ф_deployPriceXchg : XBool -> XInteger128 -> XInteger128 -> XInteger128 -> XInteger128 -> XInteger32 -> XInteger128 -> XInteger8 -> XInteger128 -> TvmCell -> addr_std_compact -> addr_std_compact -> Tip3Config -> Tip3Config -> UExpression XAddress true . 
- Parameter FLeXClient_Ф_deployWrapperWithWallet : XInteger256 -> XInteger128 -> XInteger128 -> XInteger128 -> XInteger128 -> Tip3Config -> UExpression XAddress true . 
- Parameter FLeXClient_Ф_deployEmptyFlexWallet : XInteger256 -> XInteger128 -> Tip3Config -> UExpression XAddress true . 
- Parameter FLeXClient_Ф_burnWallet : XInteger128 -> XInteger256 -> addr_std_compact -> addr_std_compact -> UExpression PhantomType true . 
- Parameter FLeXClient_Ф_getOwner : UExpression XInteger256 false . 
- Parameter FLeXClient_Ф_getFlex : UExpression XAddress false . 
- Parameter FLeXClient_Ф_hasExtWalletCode : UExpression XBool false . 
- Parameter FLeXClient_Ф_hasFlexWalletCode : UExpression XBool false . 
- Parameter FLeXClient_Ф_hasFlexWrapperCode : UExpression XBool false . 
- Parameter FLeXClient_Ф_getPayloadForDeployInternalWallet : XInteger256 -> addr_std_compact -> XInteger128 -> UExpression TvmCell false . 
- Parameter FLeXClient_Ф__fallback : UExpression TvmCell false -> UExpression XInteger false . 
+Parameter FlexClient_Ф_constructor : XInteger256 -> TvmCell -> TvmCell -> UExpression PhantomType true . 
+ Parameter FlexClient_Ф_setFlexCfg : TonsConfig -> addr_std_compact -> addr_std_compact -> UExpression PhantomType true . 
+ Parameter FlexClient_Ф_setExtWalletCode : TvmCell -> UExpression PhantomType true . 
+ Parameter FlexClient_Ф_setFlexWalletCode : TvmCell -> UExpression PhantomType true . 
+ Parameter FlexClient_Ф_setFlexWrapperCode : TvmCell -> UExpression PhantomType true . 
+ Parameter FlexClient_Ф_deployTradingPair : addr_std_compact -> XInteger128 -> XInteger128 -> XInteger128 -> UExpression XAddress true . 
+ Parameter FlexClient_Ф_deployXchgPair : addr_std_compact -> addr_std_compact -> XInteger128 -> XInteger128 -> XInteger128 -> UExpression XAddress true . 
+(*  Parameter FlexClient_Ф_preparePrice : XInteger128 -> XInteger128 -> XInteger8 -> TvmCell -> Tip3Config -> TvmCell -> UExpression ( StateInit # XAddress # XInteger256 )%type false .  *)
+ Parameter FlexClient_Ф_deployPriceWithSell : XInteger128 -> XInteger128 -> XInteger32 -> XInteger128 -> XInteger8 -> XInteger128 -> TvmCell -> addr_std_compact -> addr_std_compact -> Tip3Config -> UExpression XAddress true . 
+ Parameter FlexClient_Ф_deployPriceWithBuy : XInteger128 -> XInteger128 -> XInteger32 -> XInteger128 -> XInteger8 -> XInteger128 -> TvmCell -> addr_std_compact -> Tip3Config -> UExpression XAddress true . 
+ Parameter FlexClient_Ф_cancelSellOrder : XInteger128 -> XInteger128 -> XInteger8 -> XInteger128 -> TvmCell -> Tip3Config -> UExpression PhantomType true . 
+ Parameter FlexClient_Ф_cancelBuyOrder : XInteger128 -> XInteger128 -> XInteger8 -> XInteger128 -> TvmCell -> Tip3Config -> UExpression PhantomType true . 
+(*  Parameter FlexClient_Ф_preparePriceXchg : XInteger128 -> XInteger128 -> XInteger128 -> XInteger8 -> Tip3Config -> Tip3Config -> TvmCell -> UExpression ( StateInit # XAddress # XInteger256 )%type false .  *)
+ Parameter FlexClient_Ф_cancelXchgOrder : XBool -> XInteger128 -> XInteger128 -> XInteger128 -> XInteger8 -> XInteger128 -> TvmCell -> Tip3Config -> Tip3Config -> UExpression PhantomType true . 
+ Parameter FlexClient_Ф_transfer : addr_std_compact -> XInteger128 -> XBool -> UExpression PhantomType true . 
+ Parameter FlexClient_Ф_deployPriceXchg : XBool -> XInteger128 -> XInteger128 -> XInteger128 -> XInteger128 -> XInteger32 -> XInteger128 -> XInteger8 -> XInteger128 -> TvmCell -> addr_std_compact -> addr_std_compact -> Tip3Config -> Tip3Config -> UExpression XAddress true . 
+ Parameter FlexClient_Ф_deployWrapperWithWallet : XInteger256 -> XInteger128 -> XInteger128 -> XInteger128 -> XInteger128 -> Tip3Config -> UExpression XAddress true . 
+ Parameter FlexClient_Ф_deployEmptyFlexWallet : XInteger256 -> XInteger128 -> Tip3Config -> UExpression XAddress true . 
+ Parameter FlexClient_Ф_burnWallet : XInteger128 -> XInteger256 -> addr_std_compact -> addr_std_compact -> UExpression PhantomType true . 
+ Parameter FlexClient_Ф_getOwner : UExpression XInteger256 false . 
+ Parameter FlexClient_Ф_getFlex : UExpression XAddress false . 
+ Parameter FlexClient_Ф_hasExtWalletCode : UExpression XBool false . 
+ Parameter FlexClient_Ф_hasFlexWalletCode : UExpression XBool false . 
+ Parameter FlexClient_Ф_hasFlexWrapperCode : UExpression XBool false . 
+ Parameter FlexClient_Ф_getPayloadForDeployInternalWallet : XInteger256 -> addr_std_compact -> XInteger128 -> UExpression TvmCell false . 
+ Parameter FlexClient_Ф__fallback : UExpression TvmCell false -> UExpression XInteger false . 
 
 End specFLeXClientSig.
 
